Add derived versions of the ACL2 ASL interpreter which collect and return a trace of subprogram calls.

asllib/acl2/interp.lisp
@@ -33,14 +33,13 @@
 ;; (local (include-book "std/strings/hexify" :dir :system))
 (include-book "std/alists/alist-defuns" :dir :system)
 (local (include-book "std/lists/nth" :dir :system))
-(local (include-book "std/lists/repeat" :dir :system))
 (local (include-book "std/lists/take" :dir :system))
 (local (include-book "ihs/quotient-remainder-lemmas" :dir :system))
 (local (include-book "arithmetic/top" :dir :system))
 (local (include-book "std/alists/hons-assoc-equal" :dir :system))
 (local (include-book "std/alists/put-assoc-equal" :dir :system))
-(local (include-book "centaur/vl/util/default-hints" :dir :system))
 (local (include-book "centaur/bitops/ihsext-basics" :dir :System))
+(local (include-book "interp-theory"))
 (local (in-theory (disable floor mod unsigned-byte-p)))
 (local (table fty::deftagsum-defaults :short-names t))
 (local (in-theory (disable (tau-system))))
@@ -55,11 +54,6 @@
              (alistp x))
     :hints(("Goal" :in-theory (enable val-imap-p)))))
 
-(local
- (defthm alistp-when-func-ses-imap-p-rw
-   (implies (func-ses-imap-p x)
-            (alistp x))
-   :hints(("Goal" :in-theory (enable func-ses-imap-p)))))
 
 
 
@@ -195,18 +189,6 @@ locally, globally, or not at all"
 
 (def-env_result val_env_result-p val-p)
 (def-env_result env_env_result-p env-p)
-
-
-(local (defthm assoc-equal-is-hons-assoc-equal
-         (implies k
-                  (equal (assoc-equal k x)
-                         (hons-assoc-equal k x)))))
-
-(local (defthm identifier-p-compound-recognizer
-         (implies (identifier-p x)
-                  (stringp x))
-         :hints(("Goal" :in-theory (enable identifier-p)))
-         :rule-classes :compound-recognizer))
 
 (define val-imaplist-assoc ((key identifier-p) (stack val-imaplist-p))
   :short "Look up a variable in a stack of local storage scopes."
@@ -666,10 +648,6 @@ the wrong type."
   (val-case x
     :v_label (ev_normal x.val)
     :otherwise (ev_error "v_to_label bad type" (val-fix x) nil)))
-
-(local (defthm rationalp-when-integerp-rw
-         (implies (integerp x)
-                  (rationalp x))))
 
 
 
@@ -1382,532 +1360,630 @@ return an error."
                                                :otherwise value))))))
 
 
-(local
- (defthm constraint_kind-count-parametrized-reduction
-   (IMPLIES
-    (EQUAL (CONSTRAINT_KIND-KIND X)
-           :PARAMETRIZED)
-    (<
-     (CONSTRAINT_KIND-COUNT
-      (WELLCONSTRAINED (list (CONSTRAINT_EXACT (EXPR (E_VAR name) pos))) prec))
-     (CONSTRAINT_KIND-COUNT X)))
-   :hints(("Goal" :in-theory (enable constraint_kind-count
-                                     int_constraintlist-count
-                                     int_constraint-count
-                                     expr-count
-                                     expr_desc-count)))))
+(defthm constraint_kind-count-parametrized-reduction
+  (IMPLIES
+   (EQUAL (CONSTRAINT_KIND-KIND X)
+          :PARAMETRIZED)
+   (<
+    (CONSTRAINT_KIND-COUNT
+     (WELLCONSTRAINED (list (CONSTRAINT_EXACT (EXPR (E_VAR name) pos))) prec))
+    (CONSTRAINT_KIND-COUNT X)))
+  :hints(("Goal" :in-theory (enable constraint_kind-count
+                                    int_constraintlist-count
+                                    int_constraint-count
+                                    expr-count
+                                    expr_desc-count))))
 
 (defconst *dummy-position* (make-posn :fname "<none>" :lnum 0 :bol 0 :cnum 0))
 
 
-(with-output
-  ;; makes it so it won't take forever to print the induction scheme
-  :evisc (:gag-mode (evisc-tuple 3 4 nil nil))
-  :off (event)
-  (defines asl-interpreter-mutual-recursion
-    :short "Mutual recursion defining the ASL interpreter"
-    :parents (asl-interpreter-main-functions asl-interpreter-functions)
-    :prepwork ((local (in-theory (disable xor not)))
-               (local (xdoc::set-default-parents asl-interpreter-functions asl-interpreter-mutual-recursion)))
-    (define eval_expr ((env env-p)
-                       (e expr-p)
-                       &key
-                       ((clk natp) 'clk)
-                       (orac 'orac))
-      :parents (asl-interpreter-main-functions asl-interpreter-functions asl-interpreter-mutual-recursion)
-      :short "Evaluate an ASL expression @('e') under the given environment @('env'). Returns
+(defmacro save-form (name form)
+  `(progn
+     (defconst ,name ',form)
+     ,form))
+
+(acl2::def-b*-binder evoo
+  :parents (asl-interpreter-functions)
+  :short "The given form is expected to return two values: an @(see eval_result)
+and an @('orac'). The first value is bound with @(see patbind-evo). That is, if
+it is an error or throwing, then we return that error/thowing result and the
+@('orac'), otherwise we bind the first argument to the binder to the
+@('ev_normal->res') of the first value and continue evaluation."
+  :body
+  `(b* (((mv (evo ,(car acl2::args)) orac) . ,acl2::forms))
+     ,acl2::rest-expr))
+
+(acl2::def-b*-binder evbind
+  :parents (asl-interpreter-functions)
+  :short "Just an alias for binding @('(mv arg orac)')."
+  :body
+  `(b* (((mv ,(car acl2::args) orac) . ,acl2::forms))
+     ,acl2::rest-expr))
+
+(defmacro evo_throwing (&rest args)
+  `(mv (ev_throwing . ,args) orac))
+
+(defmacro evo-return (arg)
+  `(mv ,arg orac))
+
+(defmacro evtailcall (x) x)
+
+
+(defxdoc asl-interpreter-syntactic-requirements-for-programmatic-derivation
+  :parents (asl-interpreter-mutual-recursion)
+  :short "Syntactic conventions that need to be observed so that we can programmatically derive alternate versions of the interpreter"
+  :long "<p>It is useful to be able to derive from our original ASL interpreter (@(see
+asl-interpreter-mutual-recursion)) new versions that provide additional
+information, such as (e.g.) an execution trace (see @(see
+asl-interpreter-mutual-recursion-*t)). In order to do this easily, we need to
+follow certain conventions in the interpreter.</p>
+
+<h3>Returning Out of Interpreter Functions</h3>
+
+<p>We disallow returning values from a function with a simple @('(mv result
+orac)') form. This is because we can't tell whether it's a return from the
+function, or a return from a binding within the function, or a B*
+binding. Instead, we recognize the following forms:</p>
+
+<ul>
+<li>@('evo_normal') for returning a normal result</li>
+<li>@('evo_error') for producing an error</li>
+<li>@('evo_throwing') for throwing an exception</li>
+<li>@('evo_return') for returing an arbitrary result (may be normal, error, or throw)</li>
+<li>@('evtailcall') for a returning a direct call (tail call) of another function in the mutual recursion.</li>
+</ul>
+
+<h3>Binding Results from Non-Mutually Recursive Calls</h3>
+
+<p>Some specialized binders are used to return early in case of an error or
+throwing result from a non-mutually-recursive call. These need to be modified
+for derived functions in order to (e.g.) return additional values. Binders that don't return early </p>
+
+<ul>
+<li>@('evo') binds a single eval_result value, returns early if it is an error
+or throw</li>
+<li>@('evob') binds a single eval_result value, returns early if it is an
+error or throw but modifies the backtrace to initialize it.</li>
+</ul>
+
+<h3>Binding Results from Mutually Recursive Calls</h3>
+
+<p>Recursive calls to interpreter functions need to be bound using certain
+special B* binders. This lets us replace these binders in derived functions
+with ones that (e.g.) accept additional return values and combine them in the
+right way. We recognize the following binders for binding calls to other
+functions in the mutual recursion:</p>
+
+<ul>
+<li>@('evbind') as a replacement for a simple MV binding</li>
+<li>@('evoo') to short circuit on error and throwing results</li>
+<li>@('evs') to short circuit on error and throwing results as well as returning statement results.</li>
+</ul>
+
+<h3>Additional restrictions</h3>
+<p>These just simplify the processing of the form:</p>
+
+<ul>
+<li>Each define form has its body as the last element of the form.</li>
+<li>There is exactly one occurrence of @('///'), for the mutual recursion (none
+for the individual define forms)</li>
+<li>No auxiliary functions are defined in :prepwork.</li>
+</ul>
+")
+
+(save-form
+ *asl-interpreter-mutual-recursion-command*
+ (with-output
+   ;; makes it so it won't take forever to print the induction scheme
+   :evisc (:gag-mode (evisc-tuple 3 4 nil nil))
+   :off (event)
+   (defines asl-interpreter-mutual-recursion
+     :short "Mutual recursion defining the ASL interpreter"
+     :parents (asl-interpreter-main-functions asl-interpreter-functions)
+     :prepwork ((local (in-theory (disable xor not)))
+                (local (xdoc::set-default-parents asl-interpreter-functions asl-interpreter-mutual-recursion)))
+     (define eval_expr ((env env-p)
+                        (e expr-p)
+                        &key
+                        ((clk natp) 'clk)
+                        (orac 'orac))
+       :parents (asl-interpreter-main-functions asl-interpreter-functions asl-interpreter-mutual-recursion)
+       :short "Evaluate an ASL expression @('e') under the given environment @('env'). Returns
 an @(see eval_result) and an @('orac'). The eval_result in the @('ev_normal')
 case contains an @(see expr_result) object, consisting of the value resulting
 from evaluating the expression and a new @('env'). The global environment may
 be updated since expressions can include function calls."
-      :long "@(def eval_expr-fn)"
-      :verify-guards nil
-      :returns (mv (eval expr_eval_result-p)
-                   new-orac)
-      :measure (nats-measure clk 0 (expr-count e) 0)
-      (b* ((desc (expr->desc e))
-           (pos (expr->pos_start e)))
-        (expr_desc-case desc
-          :e_literal (evo_normal (expr_result (v_of_literal desc.val) env)) ;; SemanticsRule.ELit
-          :e_var (b* ((look (env-find desc.name env)))
-                   (env_result-case look                    ;; SemanticsRule.EVar
-                     :lk_local (evo_normal (expr_result look.val env))
-                     :lk_global (evo_normal (expr_result look.val env))
-                     :lk_notfound (evo_error "Variable not found" desc (list (list pos
-                                                                                   (local-env->storage (env->local env))
-                                                                                   (global-env->storage (env->global env)))))))
-          :e_pattern (b* (((mv (evo (expr_result v1)) orac) (eval_expr env desc.expr))
-                          ((mv (evo val) orac) (eval_pattern v1.env v1.val desc.pattern)))
-                      (evo_normal (expr_result val v1.env)))
-          :e_unop ;; anna
-          (b* (((mv (evo (expr_result v)) orac) (eval_expr env desc.arg))
-               ((evob val) (eval_unop desc.op v.val))) ;;SemanticsRule.Unop
-           (evo_normal (expr_result val v.env)))
-          :e_binop ;;
-          ;;shortcuts first
-          (case desc.op
-            (:band (b* (((mv (evo (expr_result v1)) orac) (eval_expr env desc.arg1)))
-                    (val-case v1.val
-                      :v_bool (if v1.val.val
-                                  (b* (((mv (evo (expr_result v2)) orac) (eval_expr v1.env desc.arg2))
-                                       ((evob val) (eval_binop desc.op v1.val v2.val)))
-                                    (evo_normal (expr_result val v2.env)))
-                                (evo_normal (expr_result (v_bool nil) v1.env)))
-                      :otherwise (evo_error "First argument of && evaluated to non-boolean" desc (list pos)))))
-            (:bor (b* (((mv (evo (expr_result v1)) orac) (eval_expr env desc.arg1)))
-                   (val-case v1.val
-                     :v_bool (if v1.val.val
-                                 (evo_normal (expr_result (v_bool t) v1.env))
-                               (b* (((mv (evo (expr_result v2)) orac) (eval_expr v1.env desc.arg2))
-                                    ((evob val) (eval_binop desc.op v1.val v2.val)))
-                                 (evo_normal (expr_result val v2.env))))
-                     :otherwise (evo_error "First argument of || evaluated to non-boolean" desc (list pos)))))
-            (:impl (b* (((mv (evo (expr_result v1)) orac) (eval_expr env desc.arg1)))
-                    (val-case v1.val
-                      :v_bool (if v1.val.val
-                                  (b* (((mv (evo (expr_result v2)) orac) (eval_expr v1.env desc.arg2))
-                                       ((evob val) (eval_binop desc.op v1.val v2.val)))
-                                    (evo_normal (expr_result val v2.env)))
-                                (evo_normal (expr_result (v_bool t) v1.env)))
-                      :otherwise (evo_error "First argument of ==> evaluated to non-boolean" desc (list pos)))))
-            ;;all other ops
-            (otherwise 
-             (b* (((mv (evo (expr_result v1)) orac) (eval_expr env desc.arg1))
-                  ((mv (evo (expr_result v2)) orac) (eval_expr v1.env desc.arg2))
-                  ((evob val) (eval_binop desc.op v1.val v2.val)))
-               (evo_normal (expr_result val v2.env)))))
-          :e_call ;; sol
-          (b* (((call c) desc.call)
-               ((mv (evo (exprlist_result e)) orac)
-                (eval_call c.name env c.params c.args (expr->pos_start e)))
-               (v (if (and (consp e.val)
-                           (atom (cdr e.val)))
-                      (car e.val)
-                    (v_array e.val))))
-            (evo_normal (expr_result v e.env)))
-          :e_slice ;; anna
-          (b* (((mv (evo (expr_result vexpr)) orac) (eval_expr env desc.expr))
-               ((mv (evo (intpairlist/env vslices)) orac) (eval_slice_list vexpr.env desc.slices))
-               (srcval vexpr.val)
-               )
-            (val-case srcval
-              :v_int (b* (((evob &) (check-bad-slices nil vslices.pairlist))
-                          ((intpair res) (slices_sub srcval.val vslices.pairlist)))
-                       (evo_normal
-                        (expr_result
-                         (v_bitvector res.first (loghead res.first res.second))
-                         vslices.env)))
-              :v_bitvector (b* (((evob &) (check-bad-slices srcval.len vslices.pairlist))
-                                ((intpair res) (slices_sub srcval.val vslices.pairlist)))
-                             (evo_normal
-                              (expr_result
-                               (v_bitvector res.first (loghead res.first res.second))
-                               vslices.env)))
-              :otherwise (evo_error "Unexpected result of evaluation of desc.expr" desc (list pos))))
-          :e_cond  ;; anna
-          (b* (((mv (evo (expr_result test)) orac) (eval_expr env desc.test))
-               ((evo choice) (val-case test.val
-                              :v_bool (ev_normal (if test.val.val desc.then desc.else))
-                              :otherwise (ev_error "bad test in e_cond" test.val (list pos)))))
-           (eval_expr test.env choice))
-          :e_getarray ;; sol
-          (b* (((mv (evo (expr_result arr)) orac) (eval_expr env desc.base))
-               ((mv (evo (expr_result idx)) orac) (eval_expr arr.env desc.index))
-               ((evo idxv) (val-case idx.val
-                            :v_int (ev_normal idx.val.val)
-                            :otherwise (ev_error "getarray non-integer index" desc (list pos))))
-               ((evo arrv) (val-case arr.val
-                            :v_array (ev_normal arr.val.arr)
-                            :otherwise (ev_error "getarray non-array value" desc (list pos)))))
-            (if (and (<= 0 idxv)
-                     (< idxv (len arrv)))
-                (evo_normal (expr_result (nth idxv arrv) idx.env))
-              (evo_error "getarray index out of range" desc (list pos))))
-          :e_getenumarray ;; sol
-          (b* (((mv (evo (expr_result arr)) orac) (eval_expr env desc.base))
-               ((mv (evo (expr_result idx)) orac) (eval_expr arr.env desc.index))
-               ((evo idxv) (val-case idx.val
-                             :v_label (ev_normal idx.val.val)
-                            :otherwise (ev_error "getenumarray non-label index" desc (list pos))))
-               ((evo arrv) (val-case arr.val
-                             :v_record (ev_normal arr.val.rec)
-                             :otherwise (ev_error "getenumarray non-record value" desc (list pos))))
-               (look (omap::assoc idxv arrv)))
-            (if look
-                (evo_normal (expr_result (cdr look) idx.env))
-              (evo_error "getenumarray index not found" desc (list pos))))
-          :e_getfield ;; anna
-          (b* (((mv (evo (expr_result recres)) orac) (eval_expr env desc.base))
-               ((evob fieldval) (get_field desc.field recres.val)))
-            (evo_normal (expr_result fieldval recres.env)))
-          :e_getfields ;; sol
-          (b* (((mv (evo (expr_result recres)) orac) (eval_expr env desc.base))
-               ((evob fieldvals) (map-get_field desc.fields recres.val))
-               ((evob val) (concat_bitvectors fieldvals)))
-            (evo_normal (expr_result val recres.env)))
-          :e_getcollectionfields
-          (b* (((evo gval) (env-find-global desc.base env))
-               ((evob fieldvals) (map-get_field desc.fields gval))
-               ((evob val) (concat_bitvectors fieldvals)))
-            (evo_normal (expr_result val env)))
-          :e_getitem ;; anna
-          (b* (((mv (evo (expr_result varr)) orac) (eval_expr env desc.base)))
-           (val-case varr.val
-             :v_array (if (or (< desc.index 0) (<= (len varr.val.arr) desc.index))
-                          (evo_error "index out of bounds" desc (list pos))
-                        (evo_normal (expr_result (nth desc.index varr.val.arr) varr.env)))
-             :otherwise (evo_error "evaluation of the base did not return v_array as expected" desc (list pos))))
-          :e_record ;; sol
-          (b* ((exprs (named_exprlist->exprs desc.fields))
-               (names (named_exprlist->names desc.fields))
-               ((mv (evo (exprlist_result e)) orac) (eval_expr_list env exprs)))
-            (evo_normal (expr_result (v_record (omap::from-lists names e.val)) e.env)))
-          :e_tuple ;; anna
-          (b* (((mv (evo (exprlist_result vals)) orac) (eval_expr_list env desc.exprs)))
-            (evo_normal (expr_result (v_array vals.val) vals.env)))
-          :e_array ;; sol
-          (b* (((mv (evo (expr_result v)) orac) (eval_expr env desc.value))
-               ((mv (evo (expr_result len)) orac) (eval_expr v.env desc.length))
-               ((evo lenv) (val-case len.val
-                            :v_int (if (<= 0 len.val.val)
-                                       (ev_normal len.val.val)
-                                     (ev_error "array negative length" desc (list pos)))
-                            :otherwise (ev_error "array non-integer length" desc (list pos)))))
-            (evo_normal (expr_result (v_array (make-list lenv :initial-element v.val)) len.env)))
-          :e_enumarray ;; anna
-          (b* (((mv (evo (expr_result v)) orac) (eval_expr env desc.value))
-               (labels (set::mergesort desc.labels))
-               (len (len labels))
-               (vals (make-list len :initial-element v.val)) 
-               (rec (omap::from-lists labels vals))
-               )
-            (evo_normal (expr_result (v_record rec) v.env)))
-          :e_arbitrary ;; sol
-          (b* (((mv (evo ty) orac) (resolve-ty env desc.type))
-               ((mv val orac) (ty-oracle-val ty orac))
-               ((unless val)
-                (evo_error "Unsatisfiable type in e_arbitrary" desc (list pos))))
-            (evo_normal (expr_result val env)))
-          :e_atc ;;anna
-          (b* (((mv (evo (expr_result v)) orac) (eval_expr env desc.expr))
-               ((mv (evo b) orac) (is_val_of_type v.env v.val desc.type)))
-            (if b (evo_normal v) (evo_error "DynError(DETAF" desc (list pos))))
-          )))
+       :long "@(def eval_expr-fn)"
+       :verify-guards nil
+       :returns (mv (eval expr_eval_result-p)
+                    new-orac)
+       :measure (nats-measure clk 0 (expr-count e) 0)
+       (b* ((desc (expr->desc e))
+            (pos (expr->pos_start e)))
+         (expr_desc-case desc
+           :e_literal (evo_normal (expr_result (v_of_literal desc.val) env)) ;; SemanticsRule.ELit
+           :e_var (b* ((look (env-find desc.name env)))
+                    (env_result-case look ;; SemanticsRule.EVar
+                      :lk_local (evo_normal (expr_result look.val env))
+                      :lk_global (evo_normal (expr_result look.val env))
+                      :lk_notfound (evo_error "Variable not found" desc (list (list pos
+                                                                                    (local-env->storage (env->local env))
+                                                                                    (global-env->storage (env->global env)))))))
+           :e_pattern (b* (((evoo (expr_result v1)) (eval_expr env desc.expr))
+                           ((evoo val) (eval_pattern v1.env v1.val desc.pattern)))
+                        (evo_normal (expr_result val v1.env)))
+           :e_unop ;; anna
+           (b* (((evoo (expr_result v)) (eval_expr env desc.arg))
+                ((evob val) (eval_unop desc.op v.val))) ;;SemanticsRule.Unop
+             (evo_normal (expr_result val v.env)))
+           :e_binop ;;
+           ;;shortcuts first
+           (case desc.op
+             (:band (b* (((evoo (expr_result v1)) (eval_expr env desc.arg1)))
+                      (val-case v1.val
+                        :v_bool (if v1.val.val
+                                    (b* (((evoo (expr_result v2)) (eval_expr v1.env desc.arg2))
+                                         ((evob val) (eval_binop desc.op v1.val v2.val)))
+                                      (evo_normal (expr_result val v2.env)))
+                                  (evo_normal (expr_result (v_bool nil) v1.env)))
+                        :otherwise (evo_error "First argument of && evaluated to non-boolean" desc (list pos)))))
+             (:bor (b* (((evoo (expr_result v1)) (eval_expr env desc.arg1)))
+                     (val-case v1.val
+                       :v_bool (if v1.val.val
+                                   (evo_normal (expr_result (v_bool t) v1.env))
+                                 (b* (((evoo (expr_result v2)) (eval_expr v1.env desc.arg2))
+                                      ((evob val) (eval_binop desc.op v1.val v2.val)))
+                                   (evo_normal (expr_result val v2.env))))
+                       :otherwise (evo_error "First argument of || evaluated to non-boolean" desc (list pos)))))
+             (:impl (b* (((evoo (expr_result v1)) (eval_expr env desc.arg1)))
+                      (val-case v1.val
+                        :v_bool (if v1.val.val
+                                    (b* (((evoo (expr_result v2)) (eval_expr v1.env desc.arg2))
+                                         ((evob val) (eval_binop desc.op v1.val v2.val)))
+                                      (evo_normal (expr_result val v2.env)))
+                                  (evo_normal (expr_result (v_bool t) v1.env)))
+                        :otherwise (evo_error "First argument of ==> evaluated to non-boolean" desc (list pos)))))
+             ;;all other ops
+             (otherwise 
+              (b* (((evoo (expr_result v1)) (eval_expr env desc.arg1))
+                   ((evoo (expr_result v2)) (eval_expr v1.env desc.arg2))
+                   ((evob val) (eval_binop desc.op v1.val v2.val)))
+                (evo_normal (expr_result val v2.env)))))
+           :e_call ;; sol
+           (b* (((call c) desc.call)
+                ((evoo (exprlist_result e))
+                 (eval_call c.name env c.params c.args (expr->pos_start e)))
+                (v (if (and (consp e.val)
+                            (atom (cdr e.val)))
+                       (car e.val)
+                     (v_array e.val))))
+             (evo_normal (expr_result v e.env)))
+           :e_slice ;; anna
+           (b* (((evoo (expr_result vexpr)) (eval_expr env desc.expr))
+                ((evoo (intpairlist/env vslices)) (eval_slice_list vexpr.env desc.slices))
+                (srcval vexpr.val)
+                )
+             (val-case srcval
+               :v_int (b* (((evob &) (check-bad-slices nil vslices.pairlist))
+                           ((intpair res) (slices_sub srcval.val vslices.pairlist)))
+                        (evo_normal
+                         (expr_result
+                          (v_bitvector res.first (loghead res.first res.second))
+                          vslices.env)))
+               :v_bitvector (b* (((evob &) (check-bad-slices srcval.len vslices.pairlist))
+                                 ((intpair res) (slices_sub srcval.val vslices.pairlist)))
+                              (evo_normal
+                               (expr_result
+                                (v_bitvector res.first (loghead res.first res.second))
+                                vslices.env)))
+               :otherwise (evo_error "Unexpected result of evaluation of desc.expr" desc (list pos))))
+           :e_cond ;; anna
+           (b* (((evoo (expr_result test)) (eval_expr env desc.test))
+                ((evo choice) (val-case test.val
+                                :v_bool (ev_normal (if test.val.val desc.then desc.else))
+                                :otherwise (ev_error "bad test in e_cond" test.val (list pos)))))
+             (evtailcall (eval_expr test.env choice)))
+           :e_getarray ;; sol
+           (b* (((evoo (expr_result arr)) (eval_expr env desc.base))
+                ((evoo (expr_result idx)) (eval_expr arr.env desc.index))
+                ((evo idxv) (val-case idx.val
+                              :v_int (ev_normal idx.val.val)
+                              :otherwise (ev_error "getarray non-integer index" desc (list pos))))
+                ((evo arrv) (val-case arr.val
+                              :v_array (ev_normal arr.val.arr)
+                              :otherwise (ev_error "getarray non-array value" desc (list pos)))))
+             (if (and (<= 0 idxv)
+                      (< idxv (len arrv)))
+                 (evo_normal (expr_result (nth idxv arrv) idx.env))
+               (evo_error "getarray index out of range" desc (list pos))))
+           :e_getenumarray ;; sol
+           (b* (((evoo (expr_result arr)) (eval_expr env desc.base))
+                ((evoo (expr_result idx)) (eval_expr arr.env desc.index))
+                ((evo idxv) (val-case idx.val
+                              :v_label (ev_normal idx.val.val)
+                              :otherwise (ev_error "getenumarray non-label index" desc (list pos))))
+                ((evo arrv) (val-case arr.val
+                              :v_record (ev_normal arr.val.rec)
+                              :otherwise (ev_error "getenumarray non-record value" desc (list pos))))
+                (look (omap::assoc idxv arrv)))
+             (if look
+                 (evo_normal (expr_result (cdr look) idx.env))
+               (evo_error "getenumarray index not found" desc (list pos))))
+           :e_getfield ;; anna
+           (b* (((evoo (expr_result recres)) (eval_expr env desc.base))
+                ((evob fieldval) (get_field desc.field recres.val)))
+             (evo_normal (expr_result fieldval recres.env)))
+           :e_getfields ;; sol
+           (b* (((evoo (expr_result recres)) (eval_expr env desc.base))
+                ((evob fieldvals) (map-get_field desc.fields recres.val))
+                ((evob val) (concat_bitvectors fieldvals)))
+             (evo_normal (expr_result val recres.env)))
+           :e_getcollectionfields
+           (b* (((evo gval) (env-find-global desc.base env))
+                ((evob fieldvals) (map-get_field desc.fields gval))
+                ((evob val) (concat_bitvectors fieldvals)))
+             (evo_normal (expr_result val env)))
+           :e_getitem ;; anna
+           (b* (((evoo (expr_result varr)) (eval_expr env desc.base)))
+             (val-case varr.val
+               :v_array (if (or (< desc.index 0) (<= (len varr.val.arr) desc.index))
+                            (evo_error "index out of bounds" desc (list pos))
+                          (evo_normal (expr_result (nth desc.index varr.val.arr) varr.env)))
+               :otherwise (evo_error "evaluation of the base did not return v_array as expected" desc (list pos))))
+           :e_record ;; sol
+           (b* ((exprs (named_exprlist->exprs desc.fields))
+                (names (named_exprlist->names desc.fields))
+                ((evoo (exprlist_result e)) (eval_expr_list env exprs)))
+             (evo_normal (expr_result (v_record (omap::from-lists names e.val)) e.env)))
+           :e_tuple ;; anna
+           (b* (((evoo (exprlist_result vals)) (eval_expr_list env desc.exprs)))
+             (evo_normal (expr_result (v_array vals.val) vals.env)))
+           :e_array ;; sol
+           (b* (((evoo (expr_result v)) (eval_expr env desc.value))
+                ((evoo (expr_result len)) (eval_expr v.env desc.length))
+                ((evo lenv) (val-case len.val
+                              :v_int (if (<= 0 len.val.val)
+                                         (ev_normal len.val.val)
+                                       (ev_error "array negative length" desc (list pos)))
+                              :otherwise (ev_error "array non-integer length" desc (list pos)))))
+             (evo_normal (expr_result (v_array (make-list lenv :initial-element v.val)) len.env)))
+           :e_enumarray ;; anna
+           (b* (((evoo (expr_result v)) (eval_expr env desc.value))
+                (labels (set::mergesort desc.labels))
+                (len (len labels))
+                (vals (make-list len :initial-element v.val)) 
+                (rec (omap::from-lists labels vals))
+                )
+             (evo_normal (expr_result (v_record rec) v.env)))
+           :e_arbitrary ;; sol
+           (b* (((evoo ty) (resolve-ty env desc.type))
+                ((mv val orac) (ty-oracle-val ty orac))
+                ((unless val)
+                 (evo_error "Unsatisfiable type in e_arbitrary" desc (list pos))))
+             (evo_normal (expr_result val env)))
+           :e_atc ;;anna
+           (b* (((evoo (expr_result v)) (eval_expr env desc.expr))
+                ((evoo b) (is_val_of_type v.env v.val desc.type)))
+             (if b (evo_normal v) (evo_error "DynError(DETAF" desc (list pos))))
+           )))
 
-    (define resolve-int_constraints ((env env-p)
-                                     (x int_constraintlist-p)
-                                     &key ((clk natp) 'clk) (orac 'orac))
-      :short "Resolve subexpressions in the given @(see int_constraintlist) @('x') to integer
+     (define resolve-int_constraints ((env env-p)
+                                      (x int_constraintlist-p)
+                                      (pos posn-p)
+                                      &key ((clk natp) 'clk) (orac 'orac))
+       :short "Resolve subexpressions in the given @(see int_constraintlist) @('x') to integer
 literal expressions (satisfying @(see int-literal-expr-p)), or produce an error
 if this can't be done."
-      :returns (mv (res (and (eval_result-p res)
-                             (implies (eval_result-case res :ev_normal)
-                                      (int_constraintlist-p (ev_normal->res res)))))
-                   new-orac)
-      :measure (nats-measure clk 0 (int_constraintlist-count x) 0)
-      (if (atom x)
-          (evo_normal nil)
-        (b* ((constr (int_constraint-fix (car x))))
-          (int_constraint-case constr
-            :constraint_exact (b* (((mv (evo (expr_result c)) orac) (eval_expr env constr.val)))
-                                (val-case c.val
-                                  :v_int (b* ((first  (constraint_exact (expr (e_literal (l_int c.val.val)) (expr->pos_start constr.val))))
-                                              ((mv (evo (expr_result rest)) orac)
-                                               (resolve-int_constraints env (cdr x))))
-                                           (evo_normal (cons first rest)))
-                                  :otherwise (evo_error "Constraint_exact evaluated to unexpected type" constr nil)))
-            :constraint_range (b* (((mv (evo (expr_result from)) orac) (eval_expr env constr.from))
-                                   ((mv (evo (expr_result to)) orac) (eval_expr env constr.to)))
-                                (fty::multicase
-                                  ((val-case from.val)
-                                   (val-case to.val))
-                                  ((:v_int :v_int)
-                                   (b* ((first (constraint_range
-                                                (expr (e_literal (l_int from.val.val)) (expr->pos_start constr.from))
-                                                (expr (e_literal (l_int to.val.val)) (expr->pos_start constr.to))))
-                                        ((mv (evo (expr_result rest)) orac)
-                                         (resolve-int_constraints env (cdr x))))
-                                     (evo_normal (cons first rest))))
-                                  (- (evo_error "Constraint_range evaluated to unexpected type" constr nil))))))))
+       :returns (mv (res (and (eval_result-p res)
+                              (implies (eval_result-case res :ev_normal)
+                                       (int_constraintlist-p (ev_normal->res res)))))
+                    new-orac)
+       :measure (nats-measure clk 0 (int_constraintlist-count x) 0)
+       (if (atom x)
+           (evo_normal nil)
+         (b* ((constr (int_constraint-fix (car x)))
+              (pos (posn-fix pos)))
+           (int_constraint-case constr
+             :constraint_exact (b* (((evoo (expr_result c)) (eval_expr env constr.val)))
+                                 (val-case c.val
+                                   :v_int (b* ((first  (constraint_exact (expr (e_literal (l_int c.val.val)) (expr->pos_start constr.val))))
+                                               ((evoo (expr_result rest))
+                                                (resolve-int_constraints env (cdr x) pos)))
+                                            (evo_normal (cons first rest)))
+                                   :otherwise (evo_error "Constraint_exact evaluated to unexpected type" constr (list pos))))
+             :constraint_range (b* (((evoo (expr_result from)) (eval_expr env constr.from))
+                                    ((evoo (expr_result to)) (eval_expr env constr.to)))
+                                 (fty::multicase
+                                   ((val-case from.val)
+                                    (val-case to.val))
+                                   ((:v_int :v_int)
+                                    (b* ((first (constraint_range
+                                                 (expr (e_literal (l_int from.val.val)) (expr->pos_start constr.from))
+                                                 (expr (e_literal (l_int to.val.val)) (expr->pos_start constr.to))))
+                                         ((evoo (expr_result rest))
+                                          (resolve-int_constraints env (cdr x) pos)))
+                                      (evo_normal (cons first rest))))
+                                   (- (evo_error "Constraint_range evaluated to unexpected type" constr (list pos)))))))))
 
-    (define resolve-constraint_kind ((env env-p)
-                                     (x constraint_kind-p)
-                                     &key ((clk natp) 'clk) (orac 'orac))
-      :short "Resolve subexpressions in the given @(see constraint_kind) @('x') to integer
+     (define resolve-constraint_kind ((env env-p)
+                                      (x constraint_kind-p)
+                                      (pos posn-p)
+                                      &key ((clk natp) 'clk) (orac 'orac))
+       :short "Resolve subexpressions in the given @(see constraint_kind) @('x') to integer
 literal expressions (satisfying @(see int-literal-expr-p)), or produce an error
 if this can't be done."
-      :returns (mv (res (and (eval_result-p res)
-                             (implies (eval_result-case res :ev_normal)
-                                      (constraint_kind-p (ev_normal->res res)))))
-                   new-orac)
-      :measure (nats-measure clk 0 (constraint_kind-count x) 0)
-      (constraint_kind-case x
-        :unconstrained (evo_normal (unconstrained))
-        :wellconstrained (b* (((mv (evo (expr_result constrs)) orac)
-                               (resolve-int_constraints env x.constraints)))
-                           (evo_normal (wellconstrained constrs x.flag)))
-        :parametrized (b* ((new-x (wellconstrained (list (constraint_exact (expr (e_var x.name) *dummy-position*)))
-                                                   (precision_full))))
-                        (resolve-constraint_kind env new-x))
-        :otherwise (evo_error "Can't resolve constraint_kind"
-                              (constraint_kind-fix x) nil)))
+       :returns (mv (res (and (eval_result-p res)
+                              (implies (eval_result-case res :ev_normal)
+                                       (constraint_kind-p (ev_normal->res res)))))
+                    new-orac)
+       :measure (nats-measure clk 0 (constraint_kind-count x) 0)
+       (constraint_kind-case x
+         :unconstrained (evo_normal (unconstrained))
+         :wellconstrained (b* (((evoo (expr_result constrs))
+                                (resolve-int_constraints env x.constraints pos)))
+                            (evo_normal (wellconstrained constrs x.flag)))
+         :parametrized (b* ((new-x (wellconstrained (list (constraint_exact (expr (e_var x.name) *dummy-position*)))
+                                                    (precision_full))))
+                         (evtailcall (resolve-constraint_kind env new-x pos)))
+         :otherwise (evo_error "Can't resolve constraint_kind"
+                               (constraint_kind-fix x) (list (posn-fix pos)))))
 
-    (define resolve-tylist ((env env-p)
-                            (x tylist-p)
-                            &key ((clk natp) 'clk) (orac 'orac))
-      :short "Resolve subexpressions in the given list of types (@(see tylist)) @('x') to
+     (define resolve-tylist ((env env-p)
+                             (x tylist-p)
+                             &key ((clk natp) 'clk) (orac 'orac))
+       :short "Resolve subexpressions in the given list of types (@(see tylist)) @('x') to
 integer literal expressions (satisfying @(see int-literal-expr-p)), or produce
 an error if this can't be done."
-      :returns (mv (res (and (eval_result-p res)
-                             (implies (eval_result-case res :ev_normal)
-                                      (tylist-p (ev_normal->res res)))))
-                   new-orac)
-      :measure (nats-measure clk 0 (tylist-count x) 0)
-      (if (atom x)
-          (evo_normal nil)
-        (b* (((mv (evo first) orac) (resolve-ty env (car x)))
-             ((mv (evo rest) orac) (resolve-tylist env (cdr x))))
-          (evo_normal (cons first rest)))))
+       :returns (mv (res (and (eval_result-p res)
+                              (implies (eval_result-case res :ev_normal)
+                                       (tylist-p (ev_normal->res res)))))
+                    new-orac)
+       :measure (nats-measure clk 0 (tylist-count x) 0)
+       (if (atom x)
+           (evo_normal nil)
+         (b* (((evoo first) (resolve-ty env (car x)))
+              ((evoo rest) (resolve-tylist env (cdr x))))
+           (evo_normal (cons first rest)))))
 
-    (define resolve-typed_identifierlist ((env env-p)
-                                          (x typed_identifierlist-p)
-                                          &key ((clk natp) 'clk) (orac 'orac))
-      :short "Resolve subexpressions in the given @(see typed_identifierlist)
+     (define resolve-typed_identifierlist ((env env-p)
+                                           (x typed_identifierlist-p)
+                                           &key ((clk natp) 'clk) (orac 'orac))
+       :short "Resolve subexpressions in the given @(see typed_identifierlist)
 @('x') to integer literal expressions (satisfying @(see int-literal-expr-p)),
 or produce an error if this can't be done."
-      :returns (mv (res (and (eval_result-p res)
-                             (implies (eval_result-case res :ev_normal)
-                                      (typed_identifierlist-p (ev_normal->res res)))))
-                   new-orac)
-      :measure (nats-measure clk 0 (typed_identifierlist-count x) 0)
-      (b* (((when (atom x)) (evo_normal nil))
-           ((typed_identifier x1) (car x))
-           ((mv (evo first) orac) (resolve-ty env x1.type))
-           ((mv (evo rest) orac) (resolve-typed_identifierlist env (cdr x))))
-        (evo_normal (cons (typed_identifier x1.name first) rest))))
+       :returns (mv (res (and (eval_result-p res)
+                              (implies (eval_result-case res :ev_normal)
+                                       (typed_identifierlist-p (ev_normal->res res)))))
+                    new-orac)
+       :measure (nats-measure clk 0 (typed_identifierlist-count x) 0)
+       (b* (((when (atom x)) (evo_normal nil))
+            ((typed_identifier x1) (car x))
+            ((evoo first) (resolve-ty env x1.type))
+            ((evoo rest) (resolve-typed_identifierlist env (cdr x))))
+         (evo_normal (cons (typed_identifier x1.name first) rest))))
     
-    (define resolve-ty ((env env-p)
-                        (x ty-p)
-                        &key ((clk natp) 'clk) (orac 'orac))
-      :short "Resolve subexpressions in the given type (@(see ty)) @('x') to
+     (define resolve-ty ((env env-p)
+                         (x ty-p)
+                         &key ((clk natp) 'clk) (orac 'orac))
+       :short "Resolve subexpressions in the given type (@(see ty)) @('x') to
 integer literal expressions (satisfying @(see int-literal-expr-p)), or produce
 an error if this can't be done. Used in @(see eval_expr) as part of the
 evaluation of @('e_arbitrary') expressions."
-      :returns (mv (res (and (eval_result-p res)
-                             (implies (eval_result-case res :ev_normal)
-                                      (ty-p (ev_normal->res res)))))
-                   new-orac)
-      :measure (nats-measure clk 0 (ty-count x) 0)
-      (b* ((pos (ty->pos_start x))
-           (ty (ty->desc x)))
-        (type_desc-case ty
-          :t_int (b* (((mv (evob cnstr) orac) (resolve-constraint_kind env ty.constraint)))
-                   (evo_normal (ty (t_int cnstr) pos)))
-          :t_bits (b* (((mv (evo (expr_result width)) orac) (eval_expr env ty.expr)))
-                    (val-case width.val
-                      :v_int ;;(if (<= 0 width.val.val)
-                      (evo_normal (ty (t_bits
-                                       (expr (e_literal (l_int width.val.val)) pos)
-                                       ty.fields)
-                                      pos))
-                      ;; NOTE -- separation of concerns: we once threw an error if we resolved
-                      ;; the bitvector width to a negative value. But instead we'll
-                      ;; rely on the consumer of this type to deal with it.
-                      ;; (evo_error "Negative bitvector width resolving type" x))
-                      :otherwise (evo_error "Unexpected type of bitvector width type"
-                                            (ty-fix x) (list pos))))
-          :t_tuple (b* (((mv (evo tys) orac) (resolve-tylist env ty.types)))
-                     (evo_normal (ty (t_tuple tys) pos)))
-          :t_array (b* (((mv (evo base) orac) (resolve-ty env ty.type)))
-                     (array_index-case ty.index
-                       :arraylength_expr (b* (((mv (evo (expr_result len)) orac) (eval_expr env ty.index.length)))
-                                           (val-case len.val
-                                             :v_int ;;(if (<= 0 len.val.val)
-                                             (evo_normal (ty (t_array
-                                                              (arraylength_expr
-                                                               (expr (e_literal (l_int len.val.val)) pos))
-                                                              base)
-                                                             pos))
-                                             ;; (evo_error "Negative array length resolving type" x))
-                                             :otherwise (evo_error "Unexpected type of array length"
-                                                                   (ty-fix x) (list pos))))
-                       :arraylength_enum (evo_normal (ty (t_array ty.index base) pos))))
-          :t_record (b* (((mv (evo fields) orac)
-                          (resolve-typed_identifierlist env ty.fields)))
-                      (evo_normal (ty (t_record fields) pos)))
-          :t_exception (b* (((mv (evo fields) orac)
-                             (resolve-typed_identifierlist env ty.fields)))
-                         (evo_normal (ty (t_exception fields) pos)))
-          :t_collection (b* (((mv (evo fields) orac)
-                             (resolve-typed_identifierlist env ty.fields)))
-                         (evo_normal (ty (t_collection fields) pos)))
-          :t_named  (b* ((decl_types (static_env_global->declared_types
-                                      (global-env->static (env->global env))))
-                         (look (hons-assoc-equal ty.name decl_types))
-                         ((unless look)
-                          (evo_error "Named type not found" (ty-fix x) (list pos)))
-                         ((when (zp clk))
-                          (evo_error "Clock ran out resolving named type" (ty-fix x) (list pos)))
-                         (type (ty-timeframe->ty (cdr look))))
-                      (resolve-ty env type :clk (1- clk)))
-          :otherwise (evo_normal (ty ty pos)))))
+       :returns (mv (res (and (eval_result-p res)
+                              (implies (eval_result-case res :ev_normal)
+                                       (ty-p (ev_normal->res res)))))
+                    new-orac)
+       :measure (nats-measure clk 0 (ty-count x) 0)
+       (b* ((pos (ty->pos_start x))
+            (ty (ty->desc x)))
+         (type_desc-case ty
+           :t_int (b* (((evoo cnstr) (resolve-constraint_kind env ty.constraint pos)))
+                    (evo_normal (ty (t_int cnstr) pos)))
+           :t_bits (b* (((evoo (expr_result width)) (eval_expr env ty.expr)))
+                     (val-case width.val
+                       :v_int ;;(if (<= 0 width.val.val)
+                       (evo_normal (ty (t_bits
+                                        (expr (e_literal (l_int width.val.val)) pos)
+                                        ty.fields)
+                                       pos))
+                       ;; NOTE -- separation of concerns: we once threw an error if we resolved
+                       ;; the bitvector width to a negative value. But instead we'll
+                       ;; rely on the consumer of this type to deal with it.
+                       ;; (evo_error "Negative bitvector width resolving type" x))
+                       :otherwise (evo_error "Unexpected type of bitvector width type"
+                                             (ty-fix x) (list pos))))
+           :t_tuple (b* (((evoo tys) (resolve-tylist env ty.types)))
+                      (evo_normal (ty (t_tuple tys) pos)))
+           :t_array (b* (((evoo base) (resolve-ty env ty.type)))
+                      (array_index-case ty.index
+                        :arraylength_expr (b* (((evoo (expr_result len)) (eval_expr env ty.index.length)))
+                                            (val-case len.val
+                                              :v_int ;;(if (<= 0 len.val.val)
+                                              (evo_normal (ty (t_array
+                                                               (arraylength_expr
+                                                                (expr (e_literal (l_int len.val.val)) pos))
+                                                               base)
+                                                              pos))
+                                              ;; (evo_error "Negative array length resolving type" x))
+                                              :otherwise (evo_error "Unexpected type of array length"
+                                                                    (ty-fix x) (list pos))))
+                        :arraylength_enum (evo_normal (ty (t_array ty.index base) pos))))
+           :t_record (b* (((evoo fields)
+                           (resolve-typed_identifierlist env ty.fields)))
+                       (evo_normal (ty (t_record fields) pos)))
+           :t_exception (b* (((evoo fields)
+                              (resolve-typed_identifierlist env ty.fields)))
+                          (evo_normal (ty (t_exception fields) pos)))
+           :t_collection (b* (((evoo fields)
+                               (resolve-typed_identifierlist env ty.fields)))
+                           (evo_normal (ty (t_collection fields) pos)))
+           :t_named  (b* ((decl_types (static_env_global->declared_types
+                                       (global-env->static (env->global env))))
+                          (look (hons-assoc-equal ty.name decl_types))
+                          ((unless look)
+                           (evo_error "Named type not found" (ty-fix x) (list pos)))
+                          ((when (zp clk))
+                           (evo_error "Clock ran out resolving named type" (ty-fix x) (list pos)))
+                          (type (ty-timeframe->ty (cdr look))))
+                       (evtailcall (resolve-ty env type :clk (1- clk))))
+           :otherwise (evo_normal (ty ty pos)))))
 
     
-    (define eval_pattern ((env env-p)
-                          (val val-p)
-                          (p pattern-p)
-                          &key
-                          ((clk natp) 'clk)
-                          (orac 'orac))
-      :short "Evaluate whether the @(see pattern) @('p') matches the value @('val')."
-      :measure (nats-measure clk 0 (pattern-count p) 0)
-      ;; :returns (val val-p)
-      ;; Note: this isn't supposed to produce any side effects so we'll omit
-      ;; the environment and just return the value
-      :returns (mv (eval val_result-p) new-orac)
-      (b* ((desc (pattern->desc p))
-           (pos (pattern->pos_start p)))
-        (pattern_desc-case desc
-          :pattern_all (evo_normal (v_bool t)) ;; SemanticsRule.PAll
-          :pattern_any (eval_pattern-any env val desc.patterns)
-          :pattern_geq (b* (((mv (evo (expr_result v1)) orac) (eval_expr env desc.expr)))
-                         (mv (init-backtrace (eval_binop :geq val v1.val) pos) orac))
-          :pattern_leq (b* (((mv (evo (expr_result v1)) orac) (eval_expr env desc.expr)))
-                         (mv (init-backtrace (eval_binop :leq val v1.val) pos) orac))
-          :pattern_mask  ;;We are not checking whether set/unset are consistent
-          (val-case val
-            :v_bitvector (mv (eval_pattern_mask val desc.mask) orac)
-            :otherwise (evo_error "Unsupported pattern_mask case" desc (list pos)))
-          :pattern_not (b* (((mv (evo v1) orac) (eval_pattern env val desc.pattern)))
-                         (mv (init-backtrace (eval_unop :bnot v1) pos) orac))
-          :pattern_range (b* (((mv (evo (expr_result v1)) orac) (eval_expr env desc.lower))
-                              ((mv (evo (expr_result v2)) orac) (eval_expr env desc.upper))
-                              ((evob lower) (eval_binop :geq val v1.val))
-                              ((evob upper) (eval_binop :leq val v2.val)))
-                           (mv (init-backtrace (eval_binop :band lower upper) pos) orac))
-          :pattern_single (b* (((mv (evo (expr_result v1)) orac) (eval_expr env desc.expr)))
-                            (mv (init-backtrace (eval_binop :eq_op val v1.val) pos) orac))
-          :pattern_tuple (b* ((len (len desc.patterns))
-                              ((evo vs) (val-case val
-                                         :v_array (if (eql (len val.arr) len)
-                                                      (ev_normal val.arr)
-                                                    (ev_error "pattern tuple length mismatch"
-                                                              (pattern-fix p) (list pos)))
-                                         :otherwise (ev_error "pattern tuple type mismatch"
-                                                              (pattern-fix p) (list pos)))))
-                           (eval_pattern_tuple env vs desc.patterns)))))
+     (define eval_pattern ((env env-p)
+                           (val val-p)
+                           (p pattern-p)
+                           &key
+                           ((clk natp) 'clk)
+                           (orac 'orac))
+       :short "Evaluate whether the @(see pattern) @('p') matches the value @('val')."
+       :measure (nats-measure clk 0 (pattern-count p) 0)
+       ;; :returns (val val-p)
+       ;; Note: this isn't supposed to produce any side effects so we'll omit
+       ;; the environment and just return the value
+       :returns (mv (eval val_result-p) new-orac)
+       (b* ((desc (pattern->desc p))
+            (pos (pattern->pos_start p)))
+         (pattern_desc-case desc
+           :pattern_all (evo_normal (v_bool t)) ;; SemanticsRule.PAll
+           :pattern_any (evtailcall (eval_pattern-any env val desc.patterns))
+           :pattern_geq (b* (((evoo (expr_result v1)) (eval_expr env desc.expr)))
+                          (evo-return (init-backtrace (eval_binop :geq val v1.val) pos)))
+           :pattern_leq (b* (((evoo (expr_result v1)) (eval_expr env desc.expr)))
+                          (evo-return (init-backtrace (eval_binop :leq val v1.val) pos)))
+           :pattern_mask ;;We are not checking whether set/unset are consistent
+           (val-case val
+             :v_bitvector (evo-return (eval_pattern_mask val desc.mask))
+             :otherwise (evo_error "Unsupported pattern_mask case" desc (list pos)))
+           :pattern_not (b* (((evoo v1) (eval_pattern env val desc.pattern)))
+                          (evo-return (init-backtrace (eval_unop :bnot v1) pos)))
+           :pattern_range (b* (((evoo (expr_result v1)) (eval_expr env desc.lower))
+                               ((evoo (expr_result v2)) (eval_expr env desc.upper))
+                               ((evob lower) (eval_binop :geq val v1.val))
+                               ((evob upper) (eval_binop :leq val v2.val)))
+                            (evo-return (init-backtrace (eval_binop :band lower upper) pos)))
+           :pattern_single (b* (((evoo (expr_result v1)) (eval_expr env desc.expr)))
+                             (evo-return (init-backtrace (eval_binop :eq_op val v1.val) pos)))
+           :pattern_tuple (b* ((len (len desc.patterns))
+                               ((evo vs) (val-case val
+                                           :v_array (if (eql (len val.arr) len)
+                                                        (ev_normal val.arr)
+                                                      (ev_error "pattern tuple length mismatch"
+                                                                (pattern-fix p) (list pos)))
+                                           :otherwise (ev_error "pattern tuple type mismatch"
+                                                                (pattern-fix p) (list pos)))))
+                            (evtailcall (eval_pattern_tuple env vs desc.patterns))))))
 
-    (define eval_pattern_tuple ((env env-p)
-                                (vals vallist-p)
-                                (p patternlist-p)
-                                &key
-                                ((clk natp) 'clk)
-                                (orac 'orac))
-      :short "Evaluate whether the @(see patternlist) @('p') matches the values @('vals')."
-      :guard (eql (len vals) (len p))
-      :measure (nats-measure clk 0 (patternlist-count p) 0)
-      :returns (mv (eval val_result-p) new-orac)
-      (b* (((when (atom p)) (evo_normal (v_bool t)))
-           ((mv (evo first) orac) (eval_pattern env (car vals) (car p)))
-           ;; short circuit?
-           ((when (val-case first :v_bool (not first.val) :otherwise nil))
-            (evo_normal first))
-           ((mv (evo rest) orac) (eval_pattern_tuple env (cdr vals) (cdr p))))
-        (mv (eval_binop :band first rest) orac)))
+     (define eval_pattern_tuple ((env env-p)
+                                 (vals vallist-p)
+                                 (p patternlist-p)
+                                 &key
+                                 ((clk natp) 'clk)
+                                 (orac 'orac))
+       :short "Evaluate whether the @(see patternlist) @('p') matches the values @('vals')."
+       :guard (eql (len vals) (len p))
+       :measure (nats-measure clk 0 (patternlist-count p) 0)
+       :returns (mv (eval val_result-p) new-orac)
+       (b* (((when (atom p)) (evo_normal (v_bool t)))
+            ((evoo first) (eval_pattern env (car vals) (car p)))
+            ;; short circuit?
+            ((when (val-case first :v_bool (not first.val) :otherwise nil))
+             (evo_normal first))
+            ((evoo rest) (eval_pattern_tuple env (cdr vals) (cdr p))))
+         (evo-return (eval_binop :band first rest))))
         
     
-    (define eval_pattern-any ((env env-p)
-                              (val val-p)
-                              (p patternlist-p)
-                              &key
-                              ((clk natp) 'clk)
-                              (orac 'orac))
-      :short "Evaluate whether any pattern in @(see patternlist) @('p') matches the value @('val')."
-      :measure (nats-measure clk 0 (patternlist-count p) 0)
-      :returns (mv (eval val_result-p) new-orac)
-      (if (atom p)
-          (evo_normal (v_bool nil))
-        (b* (((mv (evo v1) orac) (eval_pattern env val (car p))))
-         (val-case v1
-           :v_bool (if v1.val
-                       (evo_normal v1)
-                     (eval_pattern-any env val (cdr p)))
-           :otherwise (evo_error "Bad result type from eval_pattern" v1 (list (pattern->pos_start (car p))))))))
+     (define eval_pattern-any ((env env-p)
+                               (val val-p)
+                               (p patternlist-p)
+                               &key
+                               ((clk natp) 'clk)
+                               (orac 'orac))
+       :short "Evaluate whether any pattern in @(see patternlist) @('p') matches the value @('val')."
+       :measure (nats-measure clk 0 (patternlist-count p) 0)
+       :returns (mv (eval val_result-p) new-orac)
+       (if (atom p)
+           (evo_normal (v_bool nil))
+         (b* (((evoo v1) (eval_pattern env val (car p))))
+           (val-case v1
+             :v_bool (if v1.val
+                         (evo_normal v1)
+                       (evtailcall (eval_pattern-any env val (cdr p))))
+             :otherwise (evo_error "Bad result type from eval_pattern" v1 (list (pattern->pos_start (car p))))))))
 
 
-    (define eval_expr_list ((env env-p)
-                            (e exprlist-p)
-                            &key
-                            ((clk natp) 'clk)
-                            (orac 'orac))
-      :short "Evaluate a list of expressions. Produces an eval_result and @('orac'), where in
+     (define eval_expr_list ((env env-p)
+                             (e exprlist-p)
+                             &key
+                             ((clk natp) 'clk)
+                             (orac 'orac))
+       :short "Evaluate a list of expressions. Produces an eval_result and @('orac'), where in
 the @('ev_normal') case the eval_result contains an @(see exprlist_result)
 containing the list of values of the expressions and the final env resulting
 from the evaluations."
-      :returns (mv (eval exprlist_eval_result-p) new-orac)
-      :measure (nats-measure clk 0 (exprlist-count e) 0)
-      (b* (((when (atom e))
-            (evo_normal (exprlist_result nil env)))
-           ((mv (evo (expr_result first)) orac) (eval_expr env (car e)))
-           (env first.env)
-           ((mv (evo (exprlist_result rest)) orac) (eval_expr_list env (cdr e))))
-        (evo_normal (exprlist_result (cons first.val rest.val) rest.env))))
+       :returns (mv (eval exprlist_eval_result-p) new-orac)
+       :measure (nats-measure clk 0 (exprlist-count e) 0)
+       (b* (((when (atom e))
+             (evo_normal (exprlist_result nil env)))
+            ((evoo (expr_result first)) (eval_expr env (car e)))
+            (env first.env)
+            ((evoo (exprlist_result rest)) (eval_expr_list env (cdr e))))
+         (evo_normal (exprlist_result (cons first.val rest.val) rest.env))))
   
-    (define eval_call ((name identifier-p)
-                       (env env-p)
-                       (params exprlist-p)
-                       (args exprlist-p)
-                       (pos posn-p)
-                       &key
-                       ((clk natp) 'clk)
-                       (orac 'orac))
-      :short "Evaluate the parameter and argument expressions of a call expression or
+     (define eval_call ((name identifier-p)
+                        (env env-p)
+                        (params exprlist-p)
+                        (args exprlist-p)
+                        (pos posn-p)
+                        &key
+                        ((clk natp) 'clk)
+                        (orac 'orac))
+       :short "Evaluate the parameter and argument expressions of a call expression or
 statement, and subsequently call the given subprogram on them using @(see
 eval_subprogram). The process of calling a subprogram is divided somewhat
 arbitrarily between this function and @(see eval_subprogram). In addition to
 evaluating the parameters and arguments, this function also checks the function
 recursion limit and global recursion limit @('clk'), and pushes/pops the new
 local scope from the environment."
-      :measure (nats-measure clk 0 (+ (exprlist-count params)
-                                      (exprlist-count args)) 0)
-      :returns (mv (eval exprlist_eval_result-p) new-orac)
-      (b* (((mv (evo (exprlist_result vargs)) orac) (eval_expr_list env args))
-           ((mv (evo (exprlist_result vparams)) orac) (eval_expr_list vargs.env params))
-           (env vparams.env)
-           ;; note: we check our fixed recursion limit here because this is where
-           ;; the measure will decrease provided that they haven't been exceeded
-           ((evo sub-env) (env-push-stack name env))
-           ((when (zp clk))
-            (evo_error "Recursion limit ran out" (identifier-fix name) (list (posn-fix pos))))
-           ((mv sub-res orac)
-            (eval_subprogram sub-env name vparams.val vargs.val :clk (1- clk))))
-        (eval_result-case sub-res
-          :ev_normal (b* (((func_result subprog-eval) sub-res.res)
-                          ;; (vals (read_value_from subprog-eval.val))
-                          (env (env-pop-stack name env subprog-eval.env)))
-                       (evo_normal (exprlist_result subprog-eval.vals env)))
-          :ev_throwing (b* ((env (env-pop-stack name env (env->global sub-res.env))))
-                         (mv (ev_throwing sub-res.throwdata env (cons (list (posn-fix pos)
-                                                                            (local-env->storage (env->local vparams.env))
-                                                                            (global-env->storage (env->global vparams.env)))
-                                                                      sub-res.backtrace)) orac))
-          :ev_error (mv (change-ev_error sub-res :backtrace (cons (list (posn-fix pos)
-                                                                        (local-env->storage (env->local env))
-                                                                        (global-env->storage (env->global env)))
-                                                                  sub-res.backtrace)) orac))))
+       :measure (nats-measure clk 0 (+ (exprlist-count params)
+                                       (exprlist-count args)) 0)
+       :returns (mv (eval exprlist_eval_result-p) new-orac)
+       (b* (((evoo (exprlist_result vargs)) (eval_expr_list env args))
+            ((evoo (exprlist_result vparams)) (eval_expr_list vargs.env params))
+            (env vparams.env)
+            ;; note: we check our fixed recursion limit here because this is where
+            ;; the measure will decrease provided that they haven't been exceeded
+            ((evo sub-env) (env-push-stack name env))
+            ((when (zp clk))
+             (evo_error "Recursion limit ran out" (identifier-fix name) (list (posn-fix pos))))
+            ((evbind sub-res)
+             (eval_subprogram sub-env name vparams.val vargs.val :clk (1- clk))))
+         (eval_result-case sub-res
+           :ev_normal (b* (((func_result subprog-eval) sub-res.res)
+                           ;; (vals (read_value_from subprog-eval.val))
+                           (env (env-pop-stack name env subprog-eval.env)))
+                        (evo_normal (exprlist_result subprog-eval.vals env)))
+           :ev_throwing (b* ((env (env-pop-stack name env (env->global sub-res.env))))
+                          (evo_throwing sub-res.throwdata env (cons (list (posn-fix pos)
+                                                                             (local-env->storage (env->local vparams.env))
+                                                                             (global-env->storage (env->global vparams.env)))
+                                                                       sub-res.backtrace)))
+           :ev_error (evo-return (change-ev_error sub-res :backtrace (cons (list (posn-fix pos)
+                                                                         (local-env->storage (env->local env))
+                                                                         (global-env->storage (env->global env)))
+                                                                   sub-res.backtrace))))))
 
-    (define eval_subprogram ((env env-p)
-                             (name identifier-p)
-                             (vparams vallist-p)
-                             (vargs vallist-p)
-                             &key
-                             ((clk natp) 'clk)
-                             (orac 'orac))
-      :parents (asl-interpreter-main-functions asl-interpreter-functions asl-interpreter-mutual-recursion)
-      :short "Evaluate a subprogram, calling the function named @('name') (either an ASL
+     (define eval_subprogram ((env env-p)
+                              (name identifier-p)
+                              (vparams vallist-p)
+                              (vargs vallist-p)
+                              &key
+                              ((clk natp) 'clk)
+                              (orac 'orac))
+       :parents (asl-interpreter-main-functions asl-interpreter-functions asl-interpreter-mutual-recursion)
+       :short "Evaluate a subprogram, calling the function named @('name') (either an ASL
 function or a primitive) on the given parameter and argument values
 @('vparams'), @('vargs')."
-      :long "<p>When proving theorems about an ASL function we typically target the
+       :long "<p>When proving theorems about an ASL function we typically target the
 @('eval_subprogram') of that function, since the interface is relatively
 clean (mainly, parameters and arguments are passed in as values, not
 expressions).</p>
@@ -1918,293 +1994,291 @@ environment when we produce an @('ev_throwing') result. This is done anyway by
 see the local environment in any returned object.</p>
 
 @(def eval_subprogram-fn)"
-      :measure (nats-measure clk 1 0 0)
-      :returns (mv (eval func_eval_result-p) new-orac)
-      (b* ((look (assoc-equal (identifier-fix name)
-                              (static_env_global->subprograms
-                               (global-env->static
-                                (env->global env)))))
-           (vparams (vallist-fix vparams))
-           (vargs (vallist-fix vargs))
-           ((unless look)
-            (evo_error "Subprogam not found" (identifier-fix name) nil))
-           ((func f) (func-ses->fn (cdr look)))
-           ;; ((unless (subprogram_body-case f.body :sb_asl))
-           ;;  (evo_error "Primitive subfunctions not supported" name))
+       :measure (nats-measure clk 1 0 0)
+       :returns (mv (eval func_eval_result-p) new-orac)
+       (b* ((look (assoc-equal (identifier-fix name)
+                               (static_env_global->subprograms
+                                (global-env->static
+                                 (env->global env)))))
+            (vparams (vallist-fix vparams))
+            (vargs (vallist-fix vargs))
+            ((unless look)
+             (evo_error "Subprogam not found" (identifier-fix name) nil))
+            ((func f) (func-ses->fn (cdr look)))
+            ;; ((unless (subprogram_body-case f.body :sb_asl))
+            ;;  (evo_error "Primitive subfunctions not supported" name))
 
-           ((unless (and (eql (len vparams) (len f.parameters))
-                         (eql (len vargs) (len f.args))))
-            (evo_error "Bad arity" (cons (identifier-fix name)
-                                         (if (eql (len vparams) (len f.parameters))
-                                             (list (len vargs) (len f.args))
-                                           (list (len vparams) (len f.parameters))))
-                       (list (identifier-fix name) vparams vargs)))
+            ((unless (and (eql (len vparams) (len f.parameters))
+                          (eql (len vargs) (len f.args))))
+             (evo_error "Bad arity" (cons (identifier-fix name)
+                                          (if (eql (len vparams) (len f.parameters))
+                                              (list (len vargs) (len f.args))
+                                            (list (len vparams) (len f.parameters))))
+                        (list (identifier-fix name) vparams vargs)))
          
-           ;; probably redundant but in the document
-           (env1 (change-env env :local (empty-local-env)))
-           ((mv (evo limit) orac) (eval_limit env1 f.recurse_limit))
-           ((evo &) (check_recurse_limit env1 name limit)))
-        (subprogram_body-case f.body
-          :sb_asl (b* ((arg-names (typed_identifierlist->names f.args))
-                       (param-names (maybe-typed_identifierlist->names f.parameters))
-                       (env2 (declare_local_identifiers env1 arg-names vargs))
-                       (env3 (declare_local_identifiers env2 param-names vparams))
-                       ((mv bodyres orac) (eval_stmt env3 f.body.stmt)))
-                    ;;; NOTE: To strictly comply with the ASL reference manual
-                    ;;; we should leave the throwing env alone. But it gets
-                    ;;; stripped out by env-pop-stack in eval_call, and it's
-                    ;;; convenient for reasoning to be able to prove what a
-                    ;;; throwing result equals without including the entire
-                    ;;; local environment.
-                    (eval_result-case bodyres
-                      :ev_normal (let ((bodyres bodyres.res))
-                                   (control_flow_state-case bodyres
-                                     :returning (evo_normal (func_result bodyres.vals bodyres.env))
-                                     :continuing (evo_normal (func_result nil (env->global bodyres.env)))))
-                      :ev_error (mv (change-ev_error bodyres :backtrace (cons (list (identifier-fix name) vparams vargs) bodyres.backtrace))
-                                    orac)
-                      :ev_throwing (mv (change-ev_throwing bodyres
-                                                           :env
-                                                           (change-env bodyres.env :local (empty-local-env))
-                                                           :backtrace (cons (list (identifier-fix name) vparams vargs) bodyres.backtrace))
-                                       orac)))
-          :sb_primitive (b* (((evo primres) (eval_primitive name vparams vargs)))
-                          (evo_normal (func_result primres (env->global env)))))))
+            ;; probably redundant but in the document
+            (env1 (change-env env :local (empty-local-env)))
+            ((evoo limit) (eval_limit env1 f.recurse_limit))
+            ((evo &) (check_recurse_limit env1 name limit)))
+         (subprogram_body-case f.body
+           :sb_asl (b* ((arg-names (typed_identifierlist->names f.args))
+                        (param-names (maybe-typed_identifierlist->names f.parameters))
+                        (env2 (declare_local_identifiers env1 arg-names vargs))
+                        (env3 (declare_local_identifiers env2 param-names vparams))
+                        ((evbind bodyres) (eval_stmt env3 f.body.stmt)))
+;;; NOTE: To strictly comply with the ASL reference manual
+;;; we should leave the throwing env alone. But it gets
+;;; stripped out by env-pop-stack in eval_call, and it's
+;;; convenient for reasoning to be able to prove what a
+;;; throwing result equals without including the entire
+;;; local environment.
+                     (eval_result-case bodyres
+                       :ev_normal (let ((bodyres bodyres.res))
+                                    (control_flow_state-case bodyres
+                                      :returning (evo_normal (func_result bodyres.vals bodyres.env))
+                                      :continuing (evo_normal (func_result nil (env->global bodyres.env)))))
+                       :ev_error (evo-return (change-ev_error bodyres :backtrace (cons (list (identifier-fix name) vparams vargs) bodyres.backtrace)))
+                       :ev_throwing (evo-return (change-ev_throwing bodyres
+                                                            :env
+                                                            (change-env bodyres.env :local (empty-local-env))
+                                                            :backtrace (cons (list (identifier-fix name) vparams vargs) bodyres.backtrace)))))
+           :sb_primitive (b* (((evo primres) (eval_primitive name vparams vargs)))
+                           (evo_normal (func_result primres (env->global env)))))))
 
 
-    (define eval_lexpr ((env env-p)
-                        (lx lexpr-p)
-                        (v val-p)
-                        &key
-                        ((clk natp) 'clk)
-                        (orac 'orac))
-      :short "Evaluate an assignment of a value @('v') to a left-hand side (@(see lexpr)) @('lx')."
-      :long "<p>LHS expressions include various field/slot/slice accesses. The typical
+     (define eval_lexpr ((env env-p)
+                         (lx lexpr-p)
+                         (v val-p)
+                         &key
+                         ((clk natp) 'clk)
+                         (orac 'orac))
+       :short "Evaluate an assignment of a value @('v') to a left-hand side (@(see lexpr)) @('lx')."
+       :long "<p>LHS expressions include various field/slot/slice accesses. The typical
 pattern for assigning @('<base>.<field>') is:</p>
 <nl>
 <li>Transform @('<base>') (another lexpr) into an expression @('rbase') using @(see expr_of_lexpr)</li>
 <li>Evaluate @('rbase') using @(see eval_expr), resuting in value @('rbv')</li>
 <li>Modify @('rbv') to replace its @('<field>') field with @('v'), resulting in value @('newbase')</li>
 <li>Recursively call @('eval_lexpr') to assign @('<base>') the value @('newbase').</li></nl>"
-      :returns (mv (eval env_eval_result-p) new-orac)
-      :measure (nats-measure clk 0 (lexpr-count* lx) 0)
-      (b* ((pos (lexpr->pos_start lx))
-           (lx (lexpr->desc lx)))
-        (lexpr_desc-case lx
-          :le_discard (evo_normal (env-fix env))
-          :le_var (b* ((envres (env-assign lx.name v env)))
-                    (env_result-case envres
-                      :lk_local (evo_normal envres.val)
-                      :lk_global (evo_normal envres.val)
-                      :lk_notfound (evo_error "assign to undeclared variable" lx (list pos))))
-          :le_slice (b* ((rbase (expr_of_lexpr lx.base))
-                         ((mv (evo (expr_result rbv)) orac) (eval_expr env rbase))
-                         ((mv (evo (intpairlist/env vslices)) orac) (eval_slice_list rbv.env lx.slices))
-                         ((evob &) (check_non_overlapping_slices vslices.pairlist))
-                         ((evob newbase) (write_to_bitvector vslices.pairlist v rbv.val)))
-                      (eval_lexpr vslices.env lx.base newbase))
-          :le_setarray (b* ((rbase (expr_of_lexpr lx.base))
-                            ((mv (evo (expr_result rbv)) orac) (eval_expr env rbase))
-                            ((mv (evo (expr_result idx)) orac) (eval_expr rbv.env lx.index))
-                            ((evob idxv) (v_to_int idx.val))
-                            ((evo newarray)
-                             (val-case rbv.val
-                               :v_array (if (and (<= 0 idxv)
-                                                 (< idxv (len rbv.val.arr)))
-                                            (ev_normal (v_array (update-nth idxv (val-fix v) rbv.val.arr)))
-                                          (ev_error "le_setarray index out of obunds" lx (list pos)))
-                               :otherwise (ev_error "le_setarray non array base" lx (list pos)))))
-                         (eval_lexpr idx.env lx.base newarray))
-          :le_setenumarray (b* ((rbase (expr_of_lexpr lx.base))
-                                ((mv (evo (expr_result rbv)) orac) (eval_expr env rbase))
-                                ((mv (evo (expr_result idx)) orac) (eval_expr rbv.env lx.index))
-                                ((evob idxv) (v_to_label idx.val))
-                                ((evo newarray)
-                                 (val-case rbv.val
-                                   :v_record (if (omap::assoc idxv rbv.val.rec)
-                                                 (ev_normal (v_record (omap::update idxv (val-fix v) rbv.val.rec)))
-                                               (ev_error "le_setenumarray unrecognized index" lx (list pos)))
-                                   :otherwise (ev_error "le_setenumarray non record base" lx (list pos)))))
-                             (eval_lexpr idx.env lx.base newarray))
-          :le_setfield (b* ((rbase (expr_of_lexpr lx.base))
-                            ((mv (evo (expr_result rbv)) orac) (eval_expr env rbase))
-                            ((evo newrec)
-                             (val-case rbv.val
-                               :v_record (if (omap::assoc lx.field rbv.val.rec)
-                                             (ev_normal (v_record (omap::update lx.field (val-fix v) rbv.val.rec)))
-                                           (ev_error "le_setfield unrecognized field" lx (list pos)))
-                               :otherwise (ev_error "le_setfield non record base" lx (list pos)))))
-                         (eval_lexpr rbv.env lx.base newrec))
-          :le_setfields (b* (((when (not (eql (len lx.fields) (len lx.pairs))))
-                              (evo_error "le_setfields length mismatch" lx (list pos)))
-                             (rbase (expr_of_lexpr lx.base))
-                             ((mv (evo (expr_result rbv)) orac) (eval_expr env rbase))
-                             ((evob newval) (bitvec_fields_to_record lx.fields lx.pairs rbv.val v)))
-                          (eval_lexpr rbv.env lx.base newval))
-          :le_setcollectionfields (b* (((when (not (eql (len lx.fields) (len lx.pairs))))
-                                        (evo_error "le_setfields length mismatch" lx (list pos)))
-                                       ((evo rbv) (env-find-global lx.base env))
-                                       ((evo newval) (bitvec_fields_to_record lx.fields lx.pairs rbv v))
-                                       (newenv (env-assign-global lx.base newval env)))
-                                    (evo_normal newenv))
-          :le_destructuring (val-case v
-                              :v_array (if (eql (len v.arr) (len lx.elts))
-                                           (eval_lexpr_list env lx.elts v.arr)
-                                         (evo_error "le_destructuring length mismatch" lx (list pos)))
-                              :otherwise (evo_error "le_destructuring type mismatch" lx (list pos))))))
+       :returns (mv (eval env_eval_result-p) new-orac)
+       :measure (nats-measure clk 0 (lexpr-count* lx) 0)
+       (b* ((pos (lexpr->pos_start lx))
+            (lx (lexpr->desc lx)))
+         (lexpr_desc-case lx
+           :le_discard (evo_normal (env-fix env))
+           :le_var (b* ((envres (env-assign lx.name v env)))
+                     (env_result-case envres
+                       :lk_local (evo_normal envres.val)
+                       :lk_global (evo_normal envres.val)
+                       :lk_notfound (evo_error "assign to undeclared variable" lx (list pos))))
+           :le_slice (b* ((rbase (expr_of_lexpr lx.base))
+                          ((evoo (expr_result rbv)) (eval_expr env rbase))
+                          ((evoo (intpairlist/env vslices)) (eval_slice_list rbv.env lx.slices))
+                          ((evob &) (check_non_overlapping_slices vslices.pairlist))
+                          ((evob newbase) (write_to_bitvector vslices.pairlist v rbv.val)))
+                       (evtailcall (eval_lexpr vslices.env lx.base newbase)))
+           :le_setarray (b* ((rbase (expr_of_lexpr lx.base))
+                             ((evoo (expr_result rbv)) (eval_expr env rbase))
+                             ((evoo (expr_result idx)) (eval_expr rbv.env lx.index))
+                             ((evob idxv) (v_to_int idx.val))
+                             ((evo newarray)
+                              (val-case rbv.val
+                                :v_array (if (and (<= 0 idxv)
+                                                  (< idxv (len rbv.val.arr)))
+                                             (ev_normal (v_array (update-nth idxv (val-fix v) rbv.val.arr)))
+                                           (ev_error "le_setarray index out of obunds" lx (list pos)))
+                                :otherwise (ev_error "le_setarray non array base" lx (list pos)))))
+                          (evtailcall (eval_lexpr idx.env lx.base newarray)))
+           :le_setenumarray (b* ((rbase (expr_of_lexpr lx.base))
+                                 ((evoo (expr_result rbv)) (eval_expr env rbase))
+                                 ((evoo (expr_result idx)) (eval_expr rbv.env lx.index))
+                                 ((evob idxv) (v_to_label idx.val))
+                                 ((evo newarray)
+                                  (val-case rbv.val
+                                    :v_record (if (omap::assoc idxv rbv.val.rec)
+                                                  (ev_normal (v_record (omap::update idxv (val-fix v) rbv.val.rec)))
+                                                (ev_error "le_setenumarray unrecognized index" lx (list pos)))
+                                    :otherwise (ev_error "le_setenumarray non record base" lx (list pos)))))
+                              (evtailcall (eval_lexpr idx.env lx.base newarray)))
+           :le_setfield (b* ((rbase (expr_of_lexpr lx.base))
+                             ((evoo (expr_result rbv)) (eval_expr env rbase))
+                             ((evo newrec)
+                              (val-case rbv.val
+                                :v_record (if (omap::assoc lx.field rbv.val.rec)
+                                              (ev_normal (v_record (omap::update lx.field (val-fix v) rbv.val.rec)))
+                                            (ev_error "le_setfield unrecognized field" lx (list pos)))
+                                :otherwise (ev_error "le_setfield non record base" lx (list pos)))))
+                          (evtailcall (eval_lexpr rbv.env lx.base newrec)))
+           :le_setfields (b* (((when (not (eql (len lx.fields) (len lx.pairs))))
+                               (evo_error "le_setfields length mismatch" lx (list pos)))
+                              (rbase (expr_of_lexpr lx.base))
+                              ((evoo (expr_result rbv)) (eval_expr env rbase))
+                              ((evob newval) (bitvec_fields_to_record lx.fields lx.pairs rbv.val v)))
+                           (evtailcall (eval_lexpr rbv.env lx.base newval)))
+           :le_setcollectionfields (b* (((when (not (eql (len lx.fields) (len lx.pairs))))
+                                         (evo_error "le_setfields length mismatch" lx (list pos)))
+                                        ((evo rbv) (env-find-global lx.base env))
+                                        ((evo newval) (bitvec_fields_to_record lx.fields lx.pairs rbv v))
+                                        (newenv (env-assign-global lx.base newval env)))
+                                     (evo_normal newenv))
+           :le_destructuring (val-case v
+                               :v_array (if (eql (len v.arr) (len lx.elts))
+                                            (evtailcall (eval_lexpr_list env lx.elts v.arr))
+                                          (evo_error "le_destructuring length mismatch" lx (list pos)))
+                               :otherwise (evo_error "le_destructuring type mismatch" lx (list pos))))))
 
-    (define eval_lexpr_list ((env env-p)
-                             (lx lexprlist-p)
-                             (v vallist-p)
-                             &key
-                             ((clk natp) 'clk)
-                             (orac 'orac))
-      :short "Assign a list of LHS expressions (@(see lexprlist)) @('lx') a corresponding
+     (define eval_lexpr_list ((env env-p)
+                              (lx lexprlist-p)
+                              (v vallist-p)
+                              &key
+                              ((clk natp) 'clk)
+                              (orac 'orac))
+       :short "Assign a list of LHS expressions (@(see lexprlist)) @('lx') a corresponding
 list of values @('v') using @('eval_lexpr')."
-      :guard (eql (len lx) (len v))
-      :returns (mv (eval env_eval_result-p) new-orac)
-      :measure (nats-measure clk 0 (lexprlist-count* lx) 0)
-      (b* (((when (atom lx)) (evo_normal (env-fix env)))
-           ((mv (evo env1) orac) (eval_lexpr env (car lx) (car v))))
-        (eval_lexpr_list env1 (cdr lx) (cdr v))))
+       :guard (eql (len lx) (len v))
+       :returns (mv (eval env_eval_result-p) new-orac)
+       :measure (nats-measure clk 0 (lexprlist-count* lx) 0)
+       (b* (((when (atom lx)) (evo_normal (env-fix env)))
+            ((evoo env1) (eval_lexpr env (car lx) (car v))))
+         (evtailcall (eval_lexpr_list env1 (cdr lx) (cdr v)))))
 
-    (define eval_limit ((env env-p)
-                        (x maybe-expr-p)
+     (define eval_limit ((env env-p)
+                         (x maybe-expr-p)
+                         &key
+                         ((clk natp) 'clk)
+                         (orac 'orac))
+       :short "Evaluate a loop or recursion limit, producing either an error, an integer if
+there was a limit, or nil if there was no limit."
+       :measure (nats-measure clk 0 (maybe-expr-count x) 0)
+       :returns (mv (res (and (eval_result-p res)
+                              (implies (eval_result-case res :ev_normal)
+                                       (acl2::maybe-integerp (ev_normal->res res)))))
+                    new-orac)
+       (b* (((unless x) (evo_normal nil))
+            ((evoo (expr_result res)) (eval_expr env x))
+            (pos (expr->pos_start x))
+            ((evob val) (v_to_int res.val)))
+         (evo_normal val)))
+
+     (define eval_stmt ((env env-p)
+                        (s stmt-p)
                         &key
                         ((clk natp) 'clk)
                         (orac 'orac))
-      :short "Evaluate a loop or recursion limit, producing either an error, an integer if
-there was a limit, or nil if there was no limit."
-      :measure (nats-measure clk 0 (maybe-expr-count x) 0)
-      :returns (mv (res (and (eval_result-p res)
-                             (implies (eval_result-case res :ev_normal)
-                                      (acl2::maybe-integerp (ev_normal->res res)))))
-                   new-orac)
-      (b* (((unless x) (evo_normal nil))
-           ((mv (evo (expr_result res)) orac) (eval_expr env x))
-           (pos (expr->pos_start x))
-           ((evob val) (v_to_int res.val)))
-        (evo_normal val)))
-
-    (define eval_stmt ((env env-p)
-                       (s stmt-p)
-                       &key
-                       ((clk natp) 'clk)
-                       (orac 'orac))
-      :parents (asl-interpreter-main-functions asl-interpreter-functions asl-interpreter-mutual-recursion)
-      :short "Evaluate a statement @('s') under environment @('env'). Results in an @(see
+       :parents (asl-interpreter-main-functions asl-interpreter-functions asl-interpreter-mutual-recursion)
+       :short "Evaluate a statement @('s') under environment @('env'). Results in an @(see
 eval_result) and an @('orac'), where in the @('ev_normal') case the eval_result
 contains a @(see <control_flow_state) object. This object records whether a
 return was encountered; if so, it gives the returned list of values and global
 environment, otherwise if not returning it gives the updated (full, local and
 global) environment."
-      :long "@(def eval_stmt-fn)"
-      :measure (nats-measure clk 0 (stmt-count* s) 0)
-      :returns (mv (eval stmt_eval_result-p) new-orac)
-      (b* ((pos (stmt->pos_start s))
-           (s (stmt->desc s)))
-        (stmt_desc-case s
-          :s_pass (evo_normal (continuing env))
-          :s_seq (b* (((evs env) (eval_stmt env s.first)))
-                   (eval_stmt env s.second))
-          :s_decl
-          (b* (((unless s.expr) (evo_error "uninitialized declaration" s (list pos)))
-               ((mv (evo (expr_result v)) orac) (eval_expr env s.expr)))
-            (local_decl_item-case s.item
-              :ldi_var (b* ((env (declare_local_identifier v.env s.item.name v.val)))
-                         (evo_normal (continuing env)))
-              :ldi_tuple (val-case v.val
-                           :v_array (if (eql (len v.val.arr) (len s.item.names))
-                                        (b* ((env (declare_local_identifiers v.env s.item.names v.val.arr)))
-                                          (evo_normal (continuing env)))
-                                      (evo_error "tuple length mismatch" s (list pos)))
-                           :otherwise (evo_error "local declaration type mismatch" s (list pos)))))
-          :s_assign
-          (b* (((mv (evo (expr_result v)) orac) (eval_expr env s.expr))
-               ((mv (evo new-env) orac) (eval_lexpr v.env s.lexpr v.val)))
-            (evo_normal (continuing new-env)))
-          :s_call (b* (((call c) s.call)
-                       ((mv (evo (exprlist_result cres)) orac) (eval_call c.name env c.params c.args pos)))
-                    (evo_normal (continuing cres.env)))
-          :s_return (b* (((unless s.expr)
-                          (evo_normal (returning nil (env->global env))))
-                         (x (expr->desc s.expr)))
-                      (expr_desc-case x
-                        :e_tuple
-                        ;; NOTE / WARNING: This is a deviation from the aslref/herd
-                        ;; semantics: we return a single value here for now even though
-                        ;; the official semantics is to return multiple values. This
-                        ;; distinction is important for concurrent semantics but not for
-                        ;; sequential.  The reason we made this change is that it is
-                        ;; problematic to reason about functions that might return either
-                        ;; one value or multiple. We hope to come up with a solution that
-                        ;; results in a function being consistent in the number of values
-                        ;; returned -- right now in ASL semantics a n-tuple-valued
-                        ;; function may return either N values or 1, depending on the form
-                        ;; of return statement that it reached.
-                        (b* (((mv (evo (exprlist_result xr)) orac) (eval_expr_list env x.exprs)))
-                          (evo_normal (returning (list (v_array xr.val)) (env->global xr.env))))
-                        :otherwise (b* (((mv (evo (expr_result xr)) orac) (eval_expr env s.expr)))
-                                     (evo_normal (returning (list xr.val) (env->global xr.env))))))
+       :long "@(def eval_stmt-fn)"
+       :measure (nats-measure clk 0 (stmt-count* s) 0)
+       :returns (mv (eval stmt_eval_result-p) new-orac)
+       (b* ((pos (stmt->pos_start s))
+            (s (stmt->desc s)))
+         (stmt_desc-case s
+           :s_pass (evo_normal (continuing env))
+           :s_seq (b* (((evs env) (eval_stmt env s.first)))
+                    (evtailcall (eval_stmt env s.second)))
+           :s_decl
+           (b* (((unless s.expr) (evo_error "uninitialized declaration" s (list pos)))
+                ((evoo (expr_result v)) (eval_expr env s.expr)))
+             (local_decl_item-case s.item
+               :ldi_var (b* ((env (declare_local_identifier v.env s.item.name v.val)))
+                          (evo_normal (continuing env)))
+               :ldi_tuple (val-case v.val
+                            :v_array (if (eql (len v.val.arr) (len s.item.names))
+                                         (b* ((env (declare_local_identifiers v.env s.item.names v.val.arr)))
+                                           (evo_normal (continuing env)))
+                                       (evo_error "tuple length mismatch" s (list pos)))
+                            :otherwise (evo_error "local declaration type mismatch" s (list pos)))))
+           :s_assign
+           (b* (((evoo (expr_result v)) (eval_expr env s.expr))
+                ((evoo new-env) (eval_lexpr v.env s.lexpr v.val)))
+             (evo_normal (continuing new-env)))
+           :s_call (b* (((call c) s.call)
+                        ((evoo (exprlist_result cres)) (eval_call c.name env c.params c.args pos)))
+                     (evo_normal (continuing cres.env)))
+           :s_return (b* (((unless s.expr)
+                           (evo_normal (returning nil (env->global env))))
+                          (x (expr->desc s.expr)))
+                       (expr_desc-case x
+                         :e_tuple
+                         ;; NOTE / WARNING: This is a deviation from the aslref/herd
+                         ;; semantics: we return a single value here for now even though
+                         ;; the official semantics is to return multiple values. This
+                         ;; distinction is important for concurrent semantics but not for
+                         ;; sequential.  The reason we made this change is that it is
+                         ;; problematic to reason about functions that might return either
+                         ;; one value or multiple. We hope to come up with a solution that
+                         ;; results in a function being consistent in the number of values
+                         ;; returned -- right now in ASL semantics a n-tuple-valued
+                         ;; function may return either N values or 1, depending on the form
+                         ;; of return statement that it reached.
+                         (b* (((evoo (exprlist_result xr)) (eval_expr_list env x.exprs)))
+                           (evo_normal (returning (list (v_array xr.val)) (env->global xr.env))))
+                         :otherwise (b* (((evoo (expr_result xr)) (eval_expr env s.expr)))
+                                      (evo_normal (returning (list xr.val) (env->global xr.env))))))
                          
-          :s_cond (b* (((mv (evo (expr_result test)) orac) (eval_expr env s.test))
-                       ((evo testval) (val-case test.val
-                                       :v_bool (ev_normal test.val.val)
-                                       :otherwise (ev_error "Non-boolean test result" s.test (list pos))))
-                       (next (if testval s.then s.else)))
-                    (eval_block test.env next))
-          :s_assert (b* (((mv (evo (expr_result assert)) orac) (eval_expr env s.expr)))
-                      (val-case assert.val
-                        :v_bool (if assert.val.val
-                                    (evo_normal (continuing assert.env))
-                                  (evo_error "Assertion failed" s.expr (list pos)))
-                        :otherwise (evo_error "Non-boolean assertion result" s.expr (list pos))))
-          :s_for (b* (((mv (evo (expr_result startr)) orac) (eval_expr env s.start_e))
-                      ((mv (evo (expr_result endr)) orac)   (eval_expr env s.end_e))
-                      ((mv (evo limit) orac)                (eval_limit env s.limit))
-                      (env (push_scope env))
-                      ;;; BOZO FIXME TODO: Add loop limit
-                      (env (declare_local_identifier env s.index_name startr.val))
-                      ;; Type constraints ensure that start and end are integers,
-                      ;; will do this here so we don't have to wrap them in values
-                      ((evob startv) (v_to_int startr.val))
-                      ((evob endv)   (v_to_int endr.val))
-                      ((evs env2)
-                       (eval_for env s.index_name limit
-                                      startv s.dir endv s.body))
-                      (env3 (pop_scope env2)))
-                   (evo_normal (continuing env3)))
+           :s_cond (b* (((evoo (expr_result test)) (eval_expr env s.test))
+                        ((evo testval) (val-case test.val
+                                         :v_bool (ev_normal test.val.val)
+                                         :otherwise (ev_error "Non-boolean test result" s.test (list pos))))
+                        (next (if testval s.then s.else)))
+                     (evtailcall (eval_block test.env next)))
+           :s_assert (b* (((evoo (expr_result assert)) (eval_expr env s.expr)))
+                       (val-case assert.val
+                         :v_bool (if assert.val.val
+                                     (evo_normal (continuing assert.env))
+                                   (evo_error "Assertion failed" s.expr (list pos)))
+                         :otherwise (evo_error "Non-boolean assertion result" s.expr (list pos))))
+           :s_for (b* (((evoo (expr_result startr)) (eval_expr env s.start_e))
+                       ((evoo (expr_result endr))   (eval_expr env s.end_e))
+                       ((evoo limit)                (eval_limit env s.limit))
+                       (env (push_scope env))
+;;; BOZO FIXME TODO: Add loop limit
+                       (env (declare_local_identifier env s.index_name startr.val))
+                       ;; Type constraints ensure that start and end are integers,
+                       ;; will do this here so we don't have to wrap them in values
+                       ((evob startv) (v_to_int startr.val))
+                       ((evob endv)   (v_to_int endr.val))
+                       ((evs env2)
+                        (eval_for env s.index_name limit
+                                  startv s.dir endv s.body))
+                       (env3 (pop_scope env2)))
+                    (evo_normal (continuing env3)))
                       
-          :s_while (b* (((mv (evo limit) orac) (eval_limit env s.limit)))
-                     (eval_loop env t limit s.test s.body))
-          :s_repeat (b* (((mv (evo limit) orac) (eval_limit env s.limit))
-                         ((evob limit2) (tick_loop_limit limit))
-                         ((evs env1) (eval_block env s.body)))
-                      (eval_loop env1 nil limit2 s.test s.body))
-          :s_throw (b* (((unless s.val)
-                         (mv (ev_throwing nil env (list pos)) orac))
-                        ((expr*maybe-ty s.val))
-                        ((unless s.val.ty)
-                         (evo_error "Throw with untyped exception" s (list pos)))
-                        ((mv (evo (expr_result ex)) orac) (eval_expr env s.val.expr)))
-                     (mv (ev_throwing (throwdata ex.val s.val.ty) ex.env (list pos)) orac))
-          :s_try (b* (((mv try orac) (eval_block env s.body))
-                      ((when (eval_result-case try
-                               :ev_throwing (not try.throwdata)
-                               :otherwise t))
-                       (mv try orac))
-                      ((ev_throwing try)))
-                   ;; NOTE: The eval_catchers semantics rule takes the original env (from before the eval_block above!)
-                   ;; but then uses it just for the static env, combining its static env with the dynamic env from the throw.
-                   ;; But it seems the static env shouldn't ever change so why bother?
-                   (eval_catchers try.env s.catchers s.otherwise try.throwdata try.backtrace))
+           :s_while (b* (((evoo limit) (eval_limit env s.limit)))
+                      (evtailcall (eval_loop env t limit s.test s.body)))
+           :s_repeat (b* (((evoo limit) (eval_limit env s.limit))
+                          ((evob limit2) (tick_loop_limit limit))
+                          ((evs env1) (eval_block env s.body)))
+                       (evtailcall (eval_loop env1 nil limit2 s.test s.body)))
+           :s_throw (b* (((unless s.val)
+                          (evo_throwing nil env (list pos)))
+                         ((expr*maybe-ty s.val))
+                         ((unless s.val.ty)
+                          (evo_error "Throw with untyped exception" s (list pos)))
+                         ((evoo (expr_result ex)) (eval_expr env s.val.expr)))
+                      (evo_throwing (throwdata ex.val s.val.ty) ex.env (list pos)))
+           :s_try (b* (((evbind try) (eval_block env s.body))
+                       ((when (eval_result-case try
+                                :ev_throwing (not try.throwdata)
+                                :otherwise t))
+                        (evo-return try))
+                       ((ev_throwing try)))
+                    ;; NOTE: The eval_catchers semantics rule takes the original env (from before the eval_block above!)
+                    ;; but then uses it just for the static env, combining its static env with the dynamic env from the throw.
+                    ;; But it seems the static env shouldn't ever change so why bother?
+                    (evtailcall (eval_catchers try.env s.catchers s.otherwise try.throwdata try.backtrace)))
                       
-          :s_print (b* (((mv (evo (exprlist_result e)) orac) (eval_expr_list env s.args))
-                        (str (vallist-to-string e.val))
-                        (- (cw (if s.newline "~s0~%" "~s0") str)))
-                     (evo_normal (continuing e.env)))
-          :s_unreachable (evo_error "unreachable" s (list pos))
-          :s_pragma (evo_error "unsupported statement" s (list pos)))))
+           :s_print (b* (((evoo (exprlist_result e)) (eval_expr_list env s.args))
+                         (str (vallist-to-string e.val))
+                         (- (cw (if s.newline "~s0~%" "~s0") str)))
+                      (evo_normal (continuing e.env)))
+           :s_unreachable (evo_error "unreachable" s (list pos))
+           :s_pragma (evo_error "unsupported statement" s (list pos)))))
 
      (define eval_catchers ((env env-p)
                             (catchers catcherlist-p)
@@ -2216,347 +2290,335 @@ global) environment."
                             (orac 'orac))
        :short "Given data from a thrown exception, determines whether any of the catchers or
 otherwise block from a try statement apply and calls the appropriate block."
-      :returns (mv (eval stmt_eval_result-p) new-orac)
-      :measure (nats-measure clk 0 (+ (catcherlist-count* catchers)
-                                      (maybe-stmt-count* otherwise))
-                             0)
-      (b* (((throwdata throw))
-           (catcher? (find_catcher (global-env->static (env->global env)) throw.ty catchers))
-           ((unless catcher?)
-            (b* (((unless otherwise)
-                  (mv (ev_throwing (throwdata-fix throw) env backtrace) orac))
-                 ((mv blkres orac) (eval_block env otherwise)))
-              (mv (rethrow_implicit throw blkres backtrace) orac)))
-           ((catcher c) catcher?)
-           ((unless c.name)
-            (b* (((mv blkres orac) (eval_block env c.stmt)))
-              (mv (rethrow_implicit throw blkres backtrace) orac)))
-           (env2 (declare_local_identifier env c.name throw.val))
-           ((mv blkres orac)
-            (b* (((evs blkenv) (eval_block env2 c.stmt))
-                 (env3 (remove_local_identifier blkenv c.name)))
-              (evo_normal (continuing env3)))))
-        (mv (rethrow_implicit throw blkres backtrace) orac)))
+       :returns (mv (eval stmt_eval_result-p) new-orac)
+       :measure (nats-measure clk 0 (+ (catcherlist-count* catchers)
+                                       (maybe-stmt-count* otherwise))
+                              0)
+       (b* (((throwdata throw))
+            (catcher? (find_catcher (global-env->static (env->global env)) throw.ty catchers))
+            ((unless catcher?)
+             (b* (((unless otherwise)
+                   (evo_throwing (throwdata-fix throw) env backtrace))
+                  ((evbind blkres) (eval_block env otherwise)))
+               (evo-return (rethrow_implicit throw blkres backtrace))))
+            ((catcher c) catcher?)
+            ((unless c.name)
+             (b* (((evbind blkres) (eval_block env c.stmt)))
+               (evo-return (rethrow_implicit throw blkres backtrace))))
+            (env2 (declare_local_identifier env c.name throw.val))
+            ((evbind blkres)
+             (b* (((evs blkenv) (eval_block env2 c.stmt))
+                  (env3 (remove_local_identifier blkenv c.name)))
+               (evo_normal (continuing env3)))))
+         (evo-return (rethrow_implicit throw blkres backtrace))))
            
     
    
      (define eval_slice ((env env-p)
-                        (s slice-p)
-                        &key
-                        ((clk natp) 'clk)
-                        (orac 'orac))
+                         (s slice-p)
+                         &key
+                         ((clk natp) 'clk)
+                         (orac 'orac))
        :short "Evaluates a @(see slice) @('s'), producing an @(see eval_result) which in the
 @('ev_normal') case contains an @(see intpair/env) object: an @(see intpair)
 where the first element gives the LSB of the slice and the second gives the
 width of the slice, and an updated environment."
-      :returns (mv (eval slice_eval_result-p) new-orac)
-      :measure (nats-measure clk 0 (slice-count s) 0)
-      (slice-case s
-        :slice_single (b* (((mv (evo (expr_result v)) orac) (eval_expr env s.index)))
-                       (val-case v.val
-                         :v_int (evo_normal (intpair/env (intpair v.val.val 1) v.env))
-                         :otherwise (evo_error "Bad single slice"
-                                               (slice-fix s) (list (expr->pos_start s.index)))))
-        :slice_range (b* (((mv (evo (expr_result mend)) orac) (eval_expr env s.end))
-                          ((mv (evo (expr_result mstart)) orac) (eval_expr mend.env s.start)))
-                      (val-case mend.val
-                        :v_int (val-case mstart.val
-                                 :v_int (evo_normal
-                                         (intpair/env
-                                          (intpair mstart.val.val (+ 1 (- mend.val.val mstart.val.val)))
-                                          mstart.env))
-                                 :otherwise (evo_error "Bad start in the slice range" (slice-fix s)
-                                                       (list (expr->pos_start s.start))))
-                        :otherwise (evo_error "Bad top/end in the slice range"
-                                              (slice-fix s) (list (expr->pos_start s.end)))))
-        :slice_length (b* (((mv (evo (expr_result mstart)) orac) (eval_expr env s.start))
-                           ((mv (evo (expr_result mlength)) orac) (eval_expr mstart.env s.length)))
-                       (val-case mstart.val
+       :returns (mv (eval slice_eval_result-p) new-orac)
+       :measure (nats-measure clk 0 (slice-count s) 0)
+       (slice-case s
+         :slice_single (b* (((evoo (expr_result v)) (eval_expr env s.index)))
+                         (val-case v.val
+                           :v_int (evo_normal (intpair/env (intpair v.val.val 1) v.env))
+                           :otherwise (evo_error "Bad single slice"
+                                                 (slice-fix s) (list (expr->pos_start s.index)))))
+         :slice_range (b* (((evoo (expr_result mend)) (eval_expr env s.end))
+                           ((evoo (expr_result mstart)) (eval_expr mend.env s.start)))
+                        (val-case mend.val
+                          :v_int (val-case mstart.val
+                                   :v_int (evo_normal
+                                           (intpair/env
+                                            (intpair mstart.val.val (+ 1 (- mend.val.val mstart.val.val)))
+                                            mstart.env))
+                                   :otherwise (evo_error "Bad start in the slice range" (slice-fix s)
+                                                         (list (expr->pos_start s.start))))
+                          :otherwise (evo_error "Bad top/end in the slice range"
+                                                (slice-fix s) (list (expr->pos_start s.end)))))
+         :slice_length (b* (((evoo (expr_result mstart)) (eval_expr env s.start))
+                            ((evoo (expr_result mlength)) (eval_expr mstart.env s.length)))
+                         (val-case mstart.val
+                           :v_int (val-case mlength.val
+                                    :v_int (evo_normal
+                                            (intpair/env (intpair mstart.val.val mlength.val.val) mstart.env))
+                                    :otherwise (evo_error "Bad start in the slice range"
+                                                          (slice-fix s) (list (expr->pos_start s.start))))
+                           :otherwise (evo_error "Bad length in the slice range"
+                                                 (slice-fix s) (list (expr->pos_start s.length)))))
+         :slice_star (b* (((evoo (expr_result mfactor)) (eval_expr env s.factor))
+                          ((evoo (expr_result mlength)) (eval_expr mfactor.env s.length)))
+                       (val-case mfactor.val
                          :v_int (val-case mlength.val
                                   :v_int (evo_normal
-                                          (intpair/env (intpair mstart.val.val mlength.val.val) mstart.env))
-                                  :otherwise (evo_error "Bad start in the slice range"
-                                                        (slice-fix s) (list (expr->pos_start s.start))))
-                         :otherwise (evo_error "Bad length in the slice range"
-                                               (slice-fix s) (list (expr->pos_start s.length)))))
-        :slice_star (b* (((mv (evo (expr_result mfactor)) orac) (eval_expr env s.factor))
-                         ((mv (evo (expr_result mlength)) orac) (eval_expr mfactor.env s.length)))
-                     (val-case mfactor.val
-                       :v_int (val-case mlength.val
-                                :v_int (evo_normal
-                                        (intpair/env
-                                         (intpair (* mfactor.val.val mlength.val.val) mlength.val.val)
-                                         mlength.env))
-                                :otherwise (evo_error "Bad length in factor slice"
-                                                      (slice-fix s) (list (expr->pos_start s.length))))
-                       :otherwise (evo_error "Bad factor in factor slice"
-                                             (slice-fix s) (list (expr->pos_start s.factor)))))
-        ))
+                                          (intpair/env
+                                           (intpair (* mfactor.val.val mlength.val.val) mlength.val.val)
+                                           mlength.env))
+                                  :otherwise (evo_error "Bad length in factor slice"
+                                                        (slice-fix s) (list (expr->pos_start s.length))))
+                         :otherwise (evo_error "Bad factor in factor slice"
+                                               (slice-fix s) (list (expr->pos_start s.factor)))))
+         ))
      
-    (define eval_slice_list ((env env-p)
-                             (sl slicelist-p)
-                            &key
-                            ((clk natp) 'clk)
-                            (orac 'orac))
-      :short "Evaluate a list of slices with @(see eval_slice). Produces a list of @(see
+     (define eval_slice_list ((env env-p)
+                              (sl slicelist-p)
+                              &key
+                              ((clk natp) 'clk)
+                              (orac 'orac))
+       :short "Evaluate a list of slices with @(see eval_slice). Produces a list of @(see
 intpair) objects and a final environment."
-      :returns (mv (eval slices_eval_result-p) new-orac)
-      :measure (nats-measure clk 0 (slicelist-count sl) 0)
-      (b* (((when (atom sl))
-            (evo_normal (intpairlist/env nil env)))
-           ((mv (evo (intpair/env first)) orac) (eval_slice env (car sl)))
-           (env first.env)
-           ((mv (evo (intpairlist/env rest)) orac) (eval_slice_list env (cdr sl))))
-        (evo_normal (intpairlist/env (cons first.pair rest.pairlist) rest.env))))
+       :returns (mv (eval slices_eval_result-p) new-orac)
+       :measure (nats-measure clk 0 (slicelist-count sl) 0)
+       (b* (((when (atom sl))
+             (evo_normal (intpairlist/env nil env)))
+            ((evoo (intpair/env first)) (eval_slice env (car sl)))
+            (env first.env)
+            ((evoo (intpairlist/env rest)) (eval_slice_list env (cdr sl))))
+         (evo_normal (intpairlist/env (cons first.pair rest.pairlist) rest.env))))
 
-    (define eval_for ((env env-p)
-                      (index_name identifier-p)
-                      (limit acl2::maybe-integerp)
-                      (v_start integerp)
-                      (dir for_direction-p)
-                      (v_end   integerp)
-                      (body stmt-p)
-                      &key
-                      ((clk natp) 'clk)
-                      (orac 'orac))
-      :short "Evaluate a for loop. ASL semantics say the starting and ending indices are
-evaluated once, and while the index variable is set to each consecutive value
-it can't be modified, so the number of runs of the body is fixed at the
-beginning (except for the cases of returns and exceptions/errors)."
-      :measure (nats-measure clk 0
-                             (stmt-count* body)
-                             (for_loop-measure v_start v_end dir))
-      :returns (mv (eval stmt_eval_result-p) new-orac)
-      (b* (((evo limit1) (tick_loop_limit limit))
-           ((when (for_loop-test v_start v_end dir))
-            (evo_normal (continuing env)))
-           ((evs env1) (eval_block env body))
-           ((mv v_step env2) (eval_for_step env1 index_name v_start dir)))
-        (eval_for env2 index_name limit1 v_step dir v_end body)))
-
-    (define eval_loop ((env env-p)
-                       (is_while booleanp)
+     (define eval_for ((env env-p)
+                       (index_name identifier-p)
                        (limit acl2::maybe-integerp)
-                       (e_cond expr-p)
+                       (v_start integerp)
+                       (dir for_direction-p)
+                       (v_end   integerp)
                        (body stmt-p)
                        &key
                        ((clk natp) 'clk)
                        (orac 'orac))
-      :short "Evaluate a while or repeat loop. Until the limit runs out or the @('e_cond')
-expression evaluates to false (for while) or true (for repeat/until), evaluate
-the body and then call the loop again."
-      :measure (nats-measure clk 0 (+ (expr-count e_cond)
-                                      (stmt-count* body))
-                             2)
-      :returns (mv (eval stmt_eval_result-p) new-orac)
-      (b* (((mv (evo (expr_result cres)) orac) (eval_expr env e_cond))
-           (pos (expr->pos_start e_cond))
-           ((evob cbool) (v_to_bool cres.val))
-           ((when (xor is_while cbool))
-            (evo_normal (continuing cres.env)))
-           ((evob limit1) (tick_loop_limit limit))
-           ((evs env2) (eval_block cres.env body))
-           ((when (zp clk))
-            (evo_error "Loop limit ran out" (stmt-fix body) (list (stmt->pos_start body)))))
-        (eval_loop env2 is_while limit1 e_cond body :clk (1- clk))))
-           
-    (define eval_block ((env env-p)
-                        (x stmt-p)
+       :short "Evaluate a for loop. ASL semantics say the starting and ending indices are
+evaluated once, and while the index variable is set to each consecutive value
+it can't be modified, so the number of runs of the body is fixed at the
+beginning (except for the cases of returns and exceptions/errors)."
+       :measure (nats-measure clk 0
+                              (stmt-count* body)
+                              (for_loop-measure v_start v_end dir))
+       :returns (mv (eval stmt_eval_result-p) new-orac)
+       (b* (((evo limit1) (tick_loop_limit limit))
+            ((when (for_loop-test v_start v_end dir))
+             (evo_normal (continuing env)))
+            ((evs env1) (eval_block env body))
+            ((mv v_step env2) (eval_for_step env1 index_name v_start dir)))
+         (evtailcall (eval_for env2 index_name limit1 v_step dir v_end body))))
+
+     (define eval_loop ((env env-p)
+                        (is_while booleanp)
+                        (limit acl2::maybe-integerp)
+                        (e_cond expr-p)
+                        (body stmt-p)
                         &key
                         ((clk natp) 'clk)
                         (orac 'orac))
-      :short "Evaluate a statement in a new local scope frame. Local variables declared
+       :short "Evaluate a while or repeat loop. Until the limit runs out or the @('e_cond')
+expression evaluates to false (for while) or true (for repeat/until), evaluate
+the body and then call the loop again."
+       :measure (nats-measure clk 0 (+ (expr-count e_cond)
+                                       (stmt-count* body))
+                              2)
+       :returns (mv (eval stmt_eval_result-p) new-orac)
+       (b* (((evoo (expr_result cres)) (eval_expr env e_cond))
+            (pos (expr->pos_start e_cond))
+            ((evob cbool) (v_to_bool cres.val))
+            ((when (xor is_while cbool))
+             (evo_normal (continuing cres.env)))
+            ((evob limit1) (tick_loop_limit limit))
+            ((evs env2) (eval_block cres.env body))
+            ((when (zp clk))
+             (evo_error "Loop limit ran out" (stmt-fix body) (list (stmt->pos_start body)))))
+         (evtailcall (eval_loop env2 is_while limit1 e_cond body :clk (1- clk)))))
+           
+     (define eval_block ((env env-p)
+                         (x stmt-p)
+                         &key
+                         ((clk natp) 'clk)
+                         (orac 'orac))
+       :short "Evaluate a statement in a new local scope frame. Local variables declared
 within this statement will then disappear after the statement is completed."
-      :measure (nats-measure clk 0 (stmt-count* x) 1)
-      :returns (mv (eval stmt_eval_result-p) new-orac)
-      (b* ((env (push_scope env))
-           ((mv stmtres orac) (eval_stmt env x)))
-        (eval_result-case stmtres
-          :ev_normal (control_flow_state-case stmtres.res
-                       :returning (evo_normal stmtres.res)
-                       :continuing (evo_normal (continuing (pop_scope stmtres.res.env))))
-          :ev_throwing (mv (ev_throwing stmtres.throwdata
-                                        (pop_scope stmtres.env)
-                                        stmtres.backtrace)
-                           orac)
-          :otherwise (mv stmtres orac))))
+       :measure (nats-measure clk 0 (stmt-count* x) 1)
+       :returns (mv (eval stmt_eval_result-p) new-orac)
+       (b* ((env (push_scope env))
+            ((evbind stmtres) (eval_stmt env x)))
+         (eval_result-case stmtres
+           :ev_normal (control_flow_state-case stmtres.res
+                        :returning (evo_normal stmtres.res)
+                        :continuing (evo_normal (continuing (pop_scope stmtres.res.env))))
+           :ev_throwing (evo_throwing stmtres.throwdata
+                                         (pop_scope stmtres.env)
+                                         stmtres.backtrace)
+           :otherwise (evo-return stmtres))))
            
     
-    (define is_val_of_type_tuple ((env env-p) (vals vallist-p) (types tylist-p)
-                                  &key ((clk natp) 'clk)
-                                  (orac 'orac))
-      :short "Check whether values @('vals') each satisfy the corresponding @('types') using
+     (define is_val_of_type_tuple ((env env-p) (vals vallist-p) (types tylist-p)
+                                   &key ((clk natp) 'clk)
+                                   (orac 'orac))
+       :short "Check whether values @('vals') each satisfy the corresponding @('types') using
 @(see is_val_of_type)."
-      :guard (eql (len vals) (len types))
-      :returns (mv (res bool_eval_result-p) new-orac)
-      :measure (nats-measure clk 0 (tylist-count types) 0);;(vallist-count vals)
-      :guard-debug t
-      :verify-guards nil
-      (if (atom types)
-          (evo_normal t)
-        (b* ((v (car vals))
-             (ty (car types))
-             ((mv (evo first-ok) orac) (is_val_of_type env v ty))
-             ((unless first-ok) (evo_normal nil))
-             ((mv (evo rest_ok) orac) (is_val_of_type_tuple env (cdr vals) (cdr types)))
-             )
-          (evo_normal rest_ok))))
+       :guard (eql (len vals) (len types))
+       :returns (mv (res bool_eval_result-p) new-orac)
+       :measure (nats-measure clk 0 (tylist-count types) 0) ;;(vallist-count vals)
+       :guard-debug t
+       :verify-guards nil
+       (if (atom types)
+           (evo_normal t)
+         (b* ((v (car vals))
+              (ty (car types))
+              ((evoo first-ok) (is_val_of_type env v ty))
+              ((unless first-ok) (evo_normal nil))
+              ((evoo rest_ok) (is_val_of_type_tuple env (cdr vals) (cdr types)))
+              )
+           (evo_normal rest_ok))))
                         
       
     
-    (define check_int_constraints ((env env-p) (i integerp) (constrs int_constraintlist-p)
-                                   &key ((clk natp) 'clk) (orac 'orac))
-      :short "At least one constraint needs to be satisfied"
-      :long "<p>We assume that any expr eval is side-effect free, therefore there is no need to return env</p>"
-      :returns (mv (sat bool_eval_result-p) new-orac)
-      :measure (nats-measure clk 0 (int_constraintlist-count constrs) 0)
-      (if (atom constrs)
-          (evo_normal nil)
-        (b* ((constr (int_constraint-fix (car constrs)))
-             (i (lifix i)))
-          (int_constraint-case constr
-            :constraint_exact (b* (((mv (evo (expr_result c)) orac) (eval_expr env constr.val)))
-                                (val-case c.val
-                                  :v_int (if (equal c.val.val i)
-                                             (evo_normal t)
-                                           (check_int_constraints env i (cdr constrs)))
-                                  :otherwise (evo_error "Constraint_exact evaluated to unexpected type" constr (list (expr->pos_start constr.val)))))
-            :constraint_range (b* (((mv (evo (expr_result from)) orac) (eval_expr env constr.from))
-                                   ((mv (evo (expr_result to)) orac) (eval_expr env constr.to)))
-                                (fty::multicase
-                                  ((val-case from.val)
-                                   (val-case to.val))
-                                  ((:v_int :v_int) (if (and (<= from.val.val i)
-                                                            (<= i to.val.val))
-                                                       (evo_normal t)
-                                                     (check_int_constraints env i (cdr constrs))))
-                                  (- (evo_error "Constraint_range evaluated to unexpected type" constr (list (expr->pos_start constr.from))))))
-           ))))
+     (define check_int_constraints ((env env-p) (i integerp) (constrs int_constraintlist-p)
+                                    &key ((clk natp) 'clk) (orac 'orac))
+       :short "At least one constraint needs to be satisfied"
+       :long "<p>We assume that any expr eval is side-effect free, therefore there is no need to return env</p>"
+       :returns (mv (sat bool_eval_result-p) new-orac)
+       :measure (nats-measure clk 0 (int_constraintlist-count constrs) 0)
+       (if (atom constrs)
+           (evo_normal nil)
+         (b* ((constr (int_constraint-fix (car constrs)))
+              (i (lifix i)))
+           (int_constraint-case constr
+             :constraint_exact (b* (((evoo (expr_result c)) (eval_expr env constr.val)))
+                                 (val-case c.val
+                                   :v_int (if (equal c.val.val i)
+                                              (evo_normal t)
+                                            (check_int_constraints env i (cdr constrs)))
+                                   :otherwise (evo_error "Constraint_exact evaluated to unexpected type"
+                                                         constr (list (expr->pos_start constr.val)))))
+             :constraint_range (b* (((evoo (expr_result from)) (eval_expr env constr.from))
+                                    ((evoo (expr_result to)) (eval_expr env constr.to)))
+                                 (fty::multicase
+                                   ((val-case from.val)
+                                    (val-case to.val))
+                                   ((:v_int :v_int) (if (and (<= from.val.val i)
+                                                             (<= i to.val.val))
+                                                        (evo_normal t)
+                                                      (evtailcall (check_int_constraints env i (cdr constrs)))))
+                                   (- (evo_error "Constraint_range evaluated to unexpected type" constr (list (expr->pos_start constr.from))))))
+             ))))
     
-    (define is_val_of_type ((env env-p) (v val-p) (ty ty-p)
-                            &key ((clk natp) 'clk)
-                            (orac 'orac))
-      :short "Check whether the given value @('v') satisfies type @('ty'). Used
+     (define is_val_of_type ((env env-p) (v val-p) (ty ty-p)
+                             &key ((clk natp) 'clk)
+                             (orac 'orac))
+       :short "Check whether the given value @('v') satisfies type @('ty'). Used
  in @(see eval_expr) for the evaluation of @('e_atc') (asserting type
  conversion) expressions."
-      :long "<p>Expressions within types are typechecked to be pure/immutable, so following
+       :long "<p>Expressions within types are typechecked to be pure/immutable, so following
 ASLRef we don't return the environment.</p>"
-      :returns (mv (res bool_eval_result-p) new-orac)
-      :measure (nats-measure clk 0 (ty-count ty) 0);;(val-count v)
-      :guard-debug t
-      :verify-guards nil
-      (b* ((pos (ty->pos_start ty))
-           (ty (ty->desc ty))
-           (v (val-fix v)))
-        (fty::multicase
-          ((val-case v)
-           (type_desc-case ty))
-          ((:v_int :t_int) (constraint_kind-case ty.constraint
-                             :unconstrained (evo_normal t)        ;;INT_UNCONSTRAINED
-                             :wellconstrained (check_int_constraints env v.val ty.constraint.constraints) ;;INT_WELLCONSTRAINED
-                             :otherwise ;;pendingconstraines and parametrized are not mentioned in ASLRef????
-                             (evo_error "is_val_of_type failed - cases of int constrained not covered in ASLRef" (cons v ty) (list pos))))
-          ((-      :t_int) (constraint_kind-case ty.constraint
-                             :unconstrained (evo_normal t)        ;;INT_UNCONSTRAINED
-                             :otherwise (evo_error "is_val_of_type failed T_INT with other than v_int" (cons v ty) (list pos))))
-          ((:v_bitvector :t_bits) (b* (((mv (evo (expr_result n)) orac) (eval_expr env ty.expr)))
-                                    (val-case n.val
-                                      :v_int (evo_normal (equal n.val.val v.len))   ;;BITS
-                                      :otherwise (evo_error "is_val_of_type failed - unexpected value of e in (T_BITS e,-)" (cons v ty) (list pos)))))
-          ((:v_array :t_tuple) (b* (((unless (and (consp v.arr)
-                                                  (consp ty.types)))
-                                     (evo_error "For the case of tuple, both v-arr and ty.types must be non-empty lists" (cons v ty) (list pos)))
-                                    ((unless (eql (len v.arr) (len ty.types)))
-                                     (evo_error "is_val_of_type: value tuple of different length than type tuple" (cons v ty) (list pos))))
-                                 (is_val_of_type_tuple env v.arr ty.types)))
-          (- (evo_error "is_val_of_type: bad val type combo" (cons v ty) (list pos))))
-        ))
+       :returns (mv (res bool_eval_result-p) new-orac)
+       :measure (nats-measure clk 0 (ty-count ty) 0) ;;(val-count v)
+       :guard-debug t
+       :verify-guards nil
+       (b* ((pos (ty->pos_start ty))
+            (ty (ty->desc ty))
+            (v (val-fix v)))
+         (fty::multicase
+           ((val-case v)
+            (type_desc-case ty))
+           ((:v_int :t_int) (constraint_kind-case ty.constraint
+                              :unconstrained (evo_normal t) ;;INT_UNCONSTRAINED
+                              :wellconstrained (evtailcall (check_int_constraints env v.val ty.constraint.constraints)) ;;INT_WELLCONSTRAINED
+                              :otherwise ;;pendingconstraines and parametrized are not mentioned in ASLRef????
+                              (evo_error "is_val_of_type failed - cases of int constrained not covered in ASLRef" (cons v ty) (list pos))))
+           ((-      :t_int) (constraint_kind-case ty.constraint
+                              :unconstrained (evo_normal t) ;;INT_UNCONSTRAINED
+                              :otherwise (evo_error "is_val_of_type failed T_INT with other than v_int" (cons v ty) (list pos))))
+           ((:v_bitvector :t_bits) (b* (((evoo (expr_result n)) (eval_expr env ty.expr)))
+                                     (val-case n.val
+                                       :v_int (evo_normal (equal n.val.val v.len)) ;;BITS
+                                       :otherwise (evo_error "is_val_of_type failed - unexpected value of e in (T_BITS e,-)" (cons v ty) (list pos)))))
+           ((:v_array :t_tuple) (b* (((unless (and (consp v.arr)
+                                                   (consp ty.types)))
+                                      (evo_error "For the case of tuple, both v-arr and ty.types must be non-empty lists" (cons v ty) (list pos)))
+                                     ((unless (eql (len v.arr) (len ty.types)))
+                                      (evo_error "is_val_of_type: value tuple of different length than type tuple" (cons v ty) (list pos))))
+                                  (evtailcall (is_val_of_type_tuple env v.arr ty.types))))
+           (- (evo_error "is_val_of_type: bad val type combo" (cons v ty) (list pos))))
+         ))
 
-    ///
-    (local (make-event
-            `(in-theory (disable . ,(fgetprop 'eval_expr-fn 'acl2::recursivep nil (w state))))))
+     ///
+     (local (make-event
+             `(in-theory (disable . ,(fgetprop 'eval_expr-fn 'acl2::recursivep nil (w state))))))
 
-    (local (defthm xor-of-bool-fix
-             (equal (xor (acl2::bool-fix x) y) (xor x y))
-             :hints(("Goal" :in-theory (enable xor)))))
+     (local (defthm xor-of-bool-fix
+              (equal (xor (acl2::bool-fix x) y) (xor x y))
+              :hints(("Goal" :in-theory (enable xor)))))
 
     
                               
-    (encapsulate nil
-      (local (in-theory (e/d (maybe-expr-fix-when-some
-                              maybe-expr-some
-                              maybe-expr-some->Val)
-                             (maybe-expr-some-of-fields
-                              cons-equal
-                              len
-                              hons-assoc-equal
-                              nth update-nth))))
-      (fty::deffixequiv-mutual asl-interpreter-mutual-recursion))
+     (encapsulate nil
+       (local (in-theory (e/d (maybe-expr-fix-when-some
+                               maybe-expr-some
+                               maybe-expr-some->Val)
+                              (maybe-expr-some-of-fields
+                               cons-equal
+                               len
+                               hons-assoc-equal
+                               nth update-nth))))
+       (fty::deffixequiv-mutual asl-interpreter-mutual-recursion))
     
-    (std::defret-mutual len-of-eval_expr_list
-      (defret len-of-eval_expr_list
-        (implies (eval_result-case eval :ev_normal)
-                 (equal (len (exprlist_result->val (ev_normal->res eval)))
-                        (len e)))
-        :hints ('(:expand ((eval_expr_list env e))))
-        :fn eval_expr_list)
-      :skip-others t)
-
-    (local (defthm len-equal-0
-             (equal (equal 0 (len x))
-                    (not (consp x)))))
+     (std::defret-mutual len-of-eval_expr_list
+       (defret len-of-eval_expr_list
+         (implies (eval_result-case eval :ev_normal)
+                  (equal (len (exprlist_result->val (ev_normal->res eval)))
+                         (len e)))
+         :hints ('(:expand ((eval_expr_list env e))))
+         :fn eval_expr_list)
+       :skip-others t)
 
 
-    (std::defret-mutual resolved-p-of-resolve-ty
-      (defret resolved-p-of-<fn>
-        (implies (eval_result-case res :ev_normal)
-                 (int_constraintlist-resolved-p (ev_normal->res res)))
-        :hints ('(:expand (<call>)
-                  :in-theory (enable int_constraintlist-resolved-p
-                                     int_constraint-resolved-p
-                                     int-literal-expr-p)))
-        :fn resolve-int_constraints)
-      (defret resolved-p-of-<fn>
-        (implies (eval_result-case res :ev_normal)
-                 (constraint_kind-resolved-p (ev_normal->res res)))
-        :hints ('(:expand (<call>)
-                  :in-theory (enable constraint_kind-resolved-p)))
-        :fn resolve-constraint_kind)
+     (std::defret-mutual resolved-p-of-resolve-ty
+       (defret resolved-p-of-<fn>
+         (implies (eval_result-case res :ev_normal)
+                  (int_constraintlist-resolved-p (ev_normal->res res)))
+         :hints ('(:expand (<call>)
+                   :in-theory (enable int_constraintlist-resolved-p
+                                      int_constraint-resolved-p
+                                      int-literal-expr-p)))
+         :fn resolve-int_constraints)
+       (defret resolved-p-of-<fn>
+         (implies (eval_result-case res :ev_normal)
+                  (constraint_kind-resolved-p (ev_normal->res res)))
+         :hints ('(:expand (<call>)
+                   :in-theory (enable constraint_kind-resolved-p)))
+         :fn resolve-constraint_kind)
 
-      (defret resolved-p-of-<fn>
-        (implies (eval_result-case res :ev_normal)
-                 (tylist-resolved-p (ev_normal->res res)))
-        :hints ('(:expand (<call>)
-                  :in-theory (enable tylist-resolved-p)))
-        :fn resolve-tylist)
+       (defret resolved-p-of-<fn>
+         (implies (eval_result-case res :ev_normal)
+                  (tylist-resolved-p (ev_normal->res res)))
+         :hints ('(:expand (<call>)
+                   :in-theory (enable tylist-resolved-p)))
+         :fn resolve-tylist)
 
-      (defret resolved-p-of-<fn>
-        (implies (eval_result-case res :ev_normal)
-                 (typed_identifierlist-resolved-p (ev_normal->res res)))
-        :hints ('(:expand (<call>)
-                  :in-theory (enable typed_identifierlist-resolved-p
-                                     typed_identifier-resolved-p)))
-        :fn resolve-typed_identifierlist)
+       (defret resolved-p-of-<fn>
+         (implies (eval_result-case res :ev_normal)
+                  (typed_identifierlist-resolved-p (ev_normal->res res)))
+         :hints ('(:expand (<call>)
+                   :in-theory (enable typed_identifierlist-resolved-p
+                                      typed_identifier-resolved-p)))
+         :fn resolve-typed_identifierlist)
 
-      (defret resolved-p-of-<fn>
-        (implies (eval_result-case res :ev_normal)
-                 (ty-resolved-p (ev_normal->res res)))
-        :hints ('(:expand ((:free (clk) <call>))
-                  :in-theory (enable ty-resolved-p
-                                     array_index-resolved-p
-                                     int-literal-expr-p))
-                (and stable-under-simplificationp
-                     '(:expand ((ty-resolved-p x)))))
-        :fn resolve-ty)
-      :skip-others t)
+       (defret resolved-p-of-<fn>
+         (implies (eval_result-case res :ev_normal)
+                  (ty-resolved-p (ev_normal->res res)))
+         :hints ('(:expand ((:free (clk) <call>))
+                   :in-theory (enable ty-resolved-p
+                                      array_index-resolved-p
+                                      int-literal-expr-p))
+                 (and stable-under-simplificationp
+                      '(:expand ((ty-resolved-p x)))))
+         :fn resolve-ty)
+       :skip-others t)
     
-    (verify-guards eval_expr-fn :guard-debug t
-      :hints (("goal" :do-not-induct t)))))
-
-
-
-
-
-
-
-
+     (verify-guards eval_expr-fn :guard-debug t
+       :hints (("goal" :do-not-induct t))))))
