asllib/acl2/debug-interp.lisp
@@ -1,0 +1,618 @@
+;;****************************************************************************;;
+;;                                ASLRef                                      ;;
+;;****************************************************************************;;
+;;
+;; SPDX-FileCopyrightText: Copyright 2025 Arm Limited and/or its affiliates <open-source-office@arm.com>
+;; SPDX-License-Identifier: BSD-3-Clause
+;; 
+;;****************************************************************************;;
+;; Disclaimer:                                                                ;;
+;; This material covers both ASLv0 (viz, the existing ASL pseudocode language ;;
+;; which appears in the Arm Architecture Reference Manual) and ASLv1, a new,  ;;
+;; experimental, and as yet unreleased version of ASL.                        ;;
+;; This material is work in progress, more precisely at pre-Alpha quality as  ;;
+;; per Arm’s quality standards.                                               ;;
+;; In particular, this means that it would be premature to base any           ;;
+;; production tool development on this material.                              ;;
+;; However, any feedback, question, query and feature request would be most   ;;
+;; welcome; those can be sent to Arm’s Architecture Formal Team Lead          ;;
+;; Jade Alglave <jade.alglave@arm.com>, or by raising issues or PRs to the    ;;
+;; herdtools7 github repository.                                              ;;
+;;****************************************************************************;;
+
+(in-package "ASL")
+
+(include-book "interp")
+(include-book "std/util/defconsts" :dir :system)
+(include-book "clause-processors/just-expand" :dir :System)
+(local (include-book "interp-theory"))
+
+;; Define a new version of the interpreter that additionally collects
+;; debug/trace information according to a trace specification.
+
+;; First exercise: just collect a trace of all subprogram calls.
+
+(defxdoc asl-tracing
+  :parents (asl)
+  :short "Versions of the ASL interpreter that produce a trace of the evaluation"
+  :long "<p>The main ASL interpreter (see @(see asl-interpreter-mutual-recursion)) only
+produces the final result of the evaluation; in some cases we want to see (and
+reason about) what happened internally. Subtopics of this doc topic include
+derived versions of the ASL interpreter that produce trace objects. See @(see
+asl-trace) for the format of these objects.</p>")
+
+(deftypes asl-trace
+  (defprod asl-trace
+    :parents (asl-tracing)
+    :short "Describes an ASL subprogram call, including inputs, result, and sub-calls."
+    ((fn identifier-p)
+     (params vallist-p)
+     (args vallist-p)
+     (globals-in val-imap-p
+                 "The global storage state at the time this function was called. The resulting
+                 state is part of the result, for a normal result.")
+     (calls asl-tracelist "The list of subroutine calls within this call, in sequential order.")
+     (result eval_result-p
+             :reqfix (eval_result-case result
+                       :ev_normal (ev_normal (func_result-fix result.res))
+                       :otherwise result)))
+    :require (eval_result-case result
+               :ev_normal (func_result-p result.res)
+               :otherwise t)
+    :measure (acl2::two-nats-measure (acl2-count x) 1)
+    :layout :list)
+  (deflist asl-tracelist :elt-type asl-trace :true-listp t :elementp-of-nil nil
+    :parents (asl-tracing)
+    :short "A list of @(see asl-trace) elements."
+    :measure (acl2::two-nats-measure (acl2-count x) 0)))
+
+(local
+ (defthm true-listp-when-asl-tracelist-p
+   (implies (asl-tracelist-p x)
+            (true-listp x))
+   :rule-classes ((:rewrite :backchain-limit-lst 1))))
+
+(defthm asl-tracelist-p-of-append
+  (implies (and (asl-tracelist-p x)
+                (asl-tracelist-p y))
+           (asl-tracelist-p (append x y))))
+
+
+(local
+ (mutual-recursion
+  (defun find-form-by-car (car x)
+    (declare (xargs :mode :program))
+    (if (atom x)
+        nil
+      (if (equal (car x) car)
+          x
+        (find-form-by-car-list car x))))
+  (defun find-form-by-car-list (car x)
+    (if (atom x)
+        nil
+      (or (find-form-by-car car (car x))
+          (find-form-by-car-list car (cdr x)))))))
+
+(local (defun keep-define-forms-in-list (x)
+         (if (atom x)
+             nil
+           (if (and (consp (car x))
+                    (eq (caar x) 'define))
+               (cons (car x) (keep-define-forms-in-list (cdr x)))
+             (keep-define-forms-in-list (cdr x))))))
+
+(local (defun strip-post-/// (x)
+         (declare (xargs :mode :program))
+         (if (atom x)
+             x
+           (if (eq (car x) '///)
+               '(///)
+             (cons (strip-post-/// (car x))
+                   (strip-post-/// (cdr x)))))))
+
+(local (defun strip-xdoc (x)
+         (if (atom x)
+             x
+           (if (member-eq (car x) '(:short :long :parents))
+               (strip-xdoc (cddr x))
+             (cons (strip-xdoc (car x))
+                   (strip-xdoc (cdr x)))))))
+
+
+
+(defconsts *asl-interp-fns*
+  (acl2::strip-cadrs
+   (keep-define-forms-in-list
+    (find-form-by-car
+     'defines *asl-interpreter-mutual-recursion-command*))))
+
+
+(defmacro evo_normal-*ft (arg)
+  `(mv (ev_normal ,arg) orac trace))
+
+(define pass-error-*ft (val &optional (orac 'orac) (trace 'trace))
+  :inline t
+  :enabled t
+  (mv val orac trace))
+
+(defmacro evo_error-*ft (&rest args)
+  `(pass-error-*ft (ev_error . ,args) orac trace))
+
+(defmacro evo_throwing-*ft (&rest args)
+  `(mv (ev_throwing . ,args) orac trace))
+
+(defmacro evo-return-*ft (arg)
+  `(mv ,arg orac trace))
+
+(defmacro evtailcall-*ft (call)
+  `(b* (((evbind-*ft res) ,call))
+     (evo-return-*ft res)))
+
+(acl2::def-b*-binder evbind-*ft
+  :body
+  `(b* (((mv ,(car acl2::args) orac trace-tmp) . ,acl2::forms)
+        (trace (append trace-tmp trace)))
+     ,acl2::rest-expr))
+
+(acl2::def-b*-binder evo-*ft
+  :body
+  `(b* ((evresult ,(car acl2::forms)))
+     (eval_result-case evresult
+       :ev_normal (b* ,(and (not (eq (car acl2::args) '&))
+                           `((,(car acl2::args) evresult.res)))
+                    ,acl2::rest-expr)
+       :otherwise (mv evresult orac trace))))
+
+(acl2::def-b*-binder evoo-*ft
+  :body
+  `(b* (((evbind-*ft (evo-*ft ,(car acl2::args))) . ,acl2::forms))
+     ,acl2::rest-expr))
+
+(acl2::def-b*-binder evs-*ft
+  :body
+    `(b* (((evoo-*ft cflow) ,(car acl2::forms)))
+     (control_flow_state-case cflow
+              :returning (evo_normal-*ft cflow)
+              :continuing (b* ,(and (not (eq (car acl2::args) '&))
+                                    `((,(car acl2::args) cflow.env)))
+                            ,acl2::rest-expr))))
+
+(acl2::def-b*-binder evob-*ft
+  :body
+  `(b* ((evresult ,(car acl2::forms)))
+     (eval_result-case evresult
+       :ev_normal (b* ,(and (not (eq (car acl2::args) '&))
+                           `((,(car acl2::args) evresult.res)))
+                    ,acl2::rest-expr)
+       
+       :otherwise (pass-error-*ft (init-backtrace evresult pos) orac))))
+
+(defmacro evbody-*ft (body)
+  `(let ((trace nil))
+     ,body))
+
+
+
+(local
+ (defun pair-suffixed (syms suffix)
+   (if (atom syms)
+       nil
+     (cons (cons (car syms)
+                 (intern-in-package-of-symbol
+                  (concatenate 'string (symbol-name (car syms))
+                               (symbol-name suffix))
+                  (car syms)))
+           (pair-suffixed (cdr syms) suffix)))))
+
+(defconsts *eval-fulltrace-substitution*
+  (pair-suffixed (append *asl-interp-fns*
+                         '(evo_normal pass-error evo_error evo_throwing evo-return
+                                      evbind evoo evo evob evs evtailcall
+                                      asl-interpreter-mutual-recursion))
+                 '-*ft))
+  
+
+
+(local
+ (defconst *eval_subprogram-*ft-def*
+   '(define eval_subprogram-*ft ((env env-p)
+                                 (name identifier-p)
+                                 (vparams vallist-p)
+                                 (vargs vallist-p)
+                                 &key
+                                 ((clk natp) 'clk)
+                                 (orac 'orac))
+      :short "Full Tracing version of @(see eval_subprogram); see @(see
+asl-interpreter-mutual-recursion-*ft) for overview."
+      :measure (nats-measure clk 1 0 1)
+      :returns (mv (eval func_eval_result-p) new-orac
+                   (trace asl-tracelist-p))
+      (b* (((mv res orac trace) (eval_subprogram-*ft1 env name vparams vargs))
+           (trace (list (make-asl-trace
+                         :fn name
+                         :params vparams
+                         :args vargs
+                         :globals-in (global-env->storage (env->global env))
+                         :calls (acl2::rev trace)
+                         :result res))))
+        (mv res orac trace)))))
+
+
+(local
+ (defun find-eval_subprogram-def-and-rename (suffix x)
+   (if (atom x)
+       x
+     (case-match x
+       (('define 'eval_subprogram . rest)
+        `(define ,(intern-in-package-of-symbol
+                   (concatenate 'string "EVAL_SUBPROGRAM-" (symbol-name suffix) "1")
+                   'asl-pkg) . ,rest))
+       (& (cons (find-eval_subprogram-def-and-rename suffix (car x))
+                (find-eval_subprogram-def-and-rename suffix (cdr x))))))))
+
+(local
+ (defun add-define-to-defines (def x)
+   (if (atom x)
+       x
+     (case-match x
+       (('defines arg . rest)
+        (if (and (symbolp arg)
+                 (not (keywordp arg)))
+            `(defines ,arg ,def . ,rest)
+          `(defines ,def ,arg . ,rest)))
+       (& (cons (add-define-to-defines def (car x))
+                (add-define-to-defines def (cdr x))))))))
+
+(local
+ (defun add-trace-to-returns (x)
+   (if (atom x)
+       x
+     (case-match x
+       ((':returns x . rest)
+        `(:returns (,@x (trace asl-tracelist-p)) . ,rest))
+       (& (cons (add-trace-to-returns (car x))
+                (add-trace-to-returns (cdr x))))))))
+
+(local
+ (defun wrap-define-bodies (macro x)
+   (if (atom x)
+       x
+     (if (and (eq (car x) 'define)
+              (true-listp x))
+         (let ((len (len x)))
+           (update-nth (1- len)
+                       (list macro (nth (1- len) x))
+                       x))
+       (cons (wrap-define-bodies macro (car x))
+             (wrap-define-bodies macro (cdr x)))))))
+
+
+
+  
+
+
+
+
+
+
+(local
+ (defun eval-return-equiv-thms (names suffix wrld)
+   (if (atom names)
+       nil
+     (cons
+      (let* ((name (car names))
+             (name-mod (intern-in-package-of-symbol
+                        (concatenate 'string (symbol-name name) "-"
+                                     (if (eq name 'eval_subprogram)
+                                         (concatenate 'string (symbol-name suffix) "1")
+                                       (symbol-name suffix)))
+                        name))
+             (macro-args (macro-args name wrld))
+             (nonkey-formals (take (- (len macro-args)
+                                      (len (member '&key macro-args)))
+                                   macro-args)))
+        `(defret ,(intern-in-package-of-symbol
+                   (concatenate 'string "<FN>" "-" (symbol-name suffix) "-EQUALS-ORIGINAL")
+                   'asl-pkg)
+           (b* (((mv res-mod orac-mod &) (,name-mod . ,nonkey-formals))
+                ((mv res orac) (,name . ,nonkey-formals)))
+             (and (equal res-mod res)
+                  (equal orac-mod orac)))
+           :hints ((let ((expand (acl2::just-expand-cp-parse-hints
+                                  '((:free (,@nonkey-formals clk orac) (,name-mod . ,nonkey-formals))
+                                    (:free (,@nonkey-formals clk orac) (,name . ,nonkey-formals)))
+                                  world)))
+                     `(:computed-hint-replacement
+                       ((acl2::expand-marked))
+                       :clause-processor (acl2::mark-expands-cp
+                                          clause
+                                          '(t ;; last-only
+                                            t ;; lambdas
+                                            ,expand)))))
+           :fn ,name-mod))
+      (eval-return-equiv-thms (cdr names) suffix wrld)))))
+
+(local
+ (defun equals-original-thm (suffix wrld)
+   (let ((eval_subprogram-mod (intern-in-package-of-symbol
+                               (concatenate 'string "EVAL_SUBPROGRAM-" (symbol-name suffix))
+                               'eval_subprogram)))
+     `(std::defret-mutual
+        ,(intern-in-package-of-symbol
+          (concatenate 'string (symbol-name suffix) "-EQUALS-ORIGINAL")
+          'asl-pkg)
+        (defret ,(intern-in-package-of-symbol
+                  (concatenate 'string "EVAL_SUBPROGRAM-" (symbol-name suffix)
+                               "-EQUALS-ORIGINAL")
+                  'asl-pkg)
+          (b* (((mv res-mod orac-mod &) (,eval_subprogram-mod
+                                         env name vparams vargs))
+               ((mv res orac) (eval_subprogram env name vparams vargs)))
+            (and (equal res-mod res)
+                 (equal orac-mod orac)))
+          :hints ((let ((expand (acl2::just-expand-cp-parse-hints
+                                 '((:free (env name vparams vargs clk orac)
+                                    (,eval_subprogram-mod env name vparams vargs)))
+                                 world)))
+                    `(:computed-hint-replacement
+                      ((acl2::expand-marked))
+                      :clause-processor (acl2::mark-expands-cp
+                                         clause
+                                         '(t ;; last-only
+                                           t ;; lambdas
+                                           ,expand)))))
+          :fn ,eval_subprogram-mod)
+        . ,(eval-return-equiv-thms *asl-interp-fns* suffix wrld)))))
+
+(local
+ (defun insert-after-/// (forms x)
+   (if (atom x)
+       x
+     (if (eq (car x) '///)
+         (cons '/// forms)
+       (cons (insert-after-/// forms (car x))
+             (insert-after-/// forms (cdr x)))))))
+
+(local
+ (defun add-mutrec-xdoc (xdoc x)
+   (if (atom x)
+       x
+     (case-match x
+       (('defines name . rest)
+        `(defines ,name ,@xdoc . ,rest))
+       (& (cons (add-mutrec-xdoc xdoc (car x))
+                (add-mutrec-xdoc xdoc (cdr x))))))))
+
+(local
+ (defun add-define-xdoc (short x)
+   (declare (xargs :mode :program))
+   (if (atom x)
+       x
+     (case-match x
+       (('define name formals . rest)
+        `(define ,name ,formals
+           :short ,(acl2::template-subst short
+                                         :string-str-alist
+                                         `(("<NAME>" . ,(symbol-name name))))
+           . ,rest))
+       (& (cons (add-define-xdoc short (car x))
+                (add-define-xdoc short (cdr x))))))))
+
+
+(local (defconst *asl-*ft-xdoc*
+         '(:parents (asl-tracing)
+           :short "Modified version of @(see asl-interpreter-mutual-recursion) that collects a
+full trace of all subprogram calls."
+           :long "
+<p>This is an automatically generated derived version of the ASL interpreter,
+@(see asl-interpreter-mutual-recursion).  Each function in this mutual
+recursion returns the same two values as the analogous function in the original
+interpreter, and a third value that is an @(see asl-tracelist).</p>
+
+<p>The exception to this rule is that whereas @('eval_subprogram-*ft1') is
+derived from @(see eval_subprogram) and returns the tracelist of subprograms
+called within the subprogram call, a wrapper @('eval_subprogram-*ft') produces
+the trace for the whole subroutine call; calls of @('eval_subprogram')
+therefore get translated into calls of @('eval_subprogram-*ft') because they
+want to collect the trace including the outer subprogram call, not all the
+calls within that call.</p>
+
+<p>These functions produce the full trace of all subroutine calls, hence the
+@('*ft') suffix.</p>")))
+
+
+
+
+
+
+
+
+(local (in-theory (disable (tau-system)
+                           len assoc-equal append true-listp loghead hons-assoc-equal floor mod expt take
+                           acl2::repeat)))
+
+
+(local (xdoc::set-default-parents asl-interpreter-mutual-recursion-*ft))
+
+;; Assumptions about the syntax of the interpeter definition form:
+;;  - Only the one occurrence of ///
+;;  - No auxiliary functions defined in :prepwork
+;;  - Each define form has its body last (after all keyword args).
+
+;; ---------------------------------------------------------------------------
+;; Definition of the Full-Tracing ASL Interpreter (suffixed with *t)
+(make-event
+ (b* ((form *asl-interpreter-mutual-recursion-command*)
+      ;; Strip out the events after the /// (theorem about resolved-p-of-resolve-ty)
+      (form (strip-post-/// form))
+      ;; Strip out xdoc
+      (form (strip-xdoc form))
+      ;; Add xdoc topic for mutual recursion
+      (form (add-mutrec-xdoc *asl-*ft-xdoc* form))
+      ;; Add xdoc topic for each function
+      (form (add-define-xdoc
+             "Full Tracing version of @(see <NAME>); see @(see asl-interpreter-mutual-recursion-*ft) for overview."
+             form))
+      ;; Replace '(define eval_subprogram ...' with '(define eval_subprogram-*ft1'
+      ;; since it's going to be wrapped in a call that deals with collecting the trace data.
+      (form (find-eval_subprogram-def-and-rename '*ft form))
+      ;; Substitute function names with their -*ft suffixed forms.
+      (form (sublis *eval-fulltrace-substitution* form))
+      ;; Wrap each define body in a call of evbody-*ft.
+      (form (wrap-define-bodies 'evbody-*ft form))
+      ;; Add (trace asl-tracelist-p) to all the :returns forms.
+      (form (add-trace-to-returns form))
+      ;; Add the definition of eval_subprogram-*ft which wraps around eval_subprogram-*ft1.
+      (form (add-define-to-defines *eval_subprogram-*ft-def* form))
+      ;; Disable the functions, prove the non-trace return values equal to the originals, and verify guards.
+      (form (insert-after-///
+             (list
+              '(make-event
+                `(in-theory (disable . ,(fgetprop 'eval_expr-*ft-fn 'acl2::recursivep nil (w state)))))
+              (equals-original-thm '*ft (w state))
+              '(verify-guards eval_expr-*ft-fn))
+             form)))
+   form))
+;; ---------------------------------------------------------------------------
+
+
+
+
+
+(defprod tracespec-entry
+  :parents (asl-tracing)
+  :short "Entry describing what information should be collected in the trace for a given function."
+  ((paramsp booleanp)
+   (argsp booleanp)
+   (globalsp booleanp)
+   (resultp booleanp))
+  :layout :list)
+
+
+(local (in-theory (enable hons-assoc-equal)))
+(fty::defmap tracespec :key-type identifier :val-type tracespec-entry
+  :valp-of-nil nil :keyp-of-nil nil :true-listp t
+  :parents (asl-tracing)
+  :short "Specifies what information should be collected in the trace for a given subprogram.")
+
+
+
+
+
+
+
+
+(defconsts *eval-trace-substitution*
+  (append (pair-suffixed (append '(asl-interpreter-mutual-recursion) *asl-interp-fns*) '-*t)
+          *eval-fulltrace-substitution*))
+
+
+
+(local (defconst *asl-*t-xdoc*
+         '(:parents (asl-tracing)
+           :short "Modified version of @(see asl-interpreter-mutual-recursion) that collects a
+trace of a specified set of subprogram calls."
+           :long "
+<p>This is an automatically generated derived version of the ASL interpreter,
+@(see asl-interpreter-mutual-recursion).  Each function in this mutual
+recursion returns the same two values as the analogous function in the original
+interpreter, and a third value that is an @(see asl-tracelist).</p>
+
+<p>The exception to this rule is that whereas @('eval_subprogram-*t1') is
+derived from @(see eval_subprogram) and returns the tracelist of subprograms
+called within the subprogram call, a wrapper @('eval_subprogram-*t') produces
+the trace for the whole subroutine call; calls of @('eval_subprogram')
+therefore get translated into calls of @('eval_subprogram-*ft') because they
+want to collect the trace including the outer subprogram call, not all the
+calls within that call.</p>
+
+<p>These functions produce a trace as specified by an added @(see tracespec)
+argument. For each subprogram call, if that subprogram has an entry in the
+tracespec, then it produces a trace entry with information populated or elided
+according to the @(see tracespec-entry) it is mapped to. Otherwise, it returns
+the trace of any sub-calls within the body that are traced according to the
+tracespec.</p>")))
+
+(local
+ (defconst *eval_subprogram-*t-def*
+   '(define eval_subprogram-*t ((env env-p)
+                                 (name identifier-p)
+                                 (vparams vallist-p)
+                                 (vargs vallist-p)
+                                 &key
+                                 ((clk natp) 'clk)
+                                 (orac 'orac)
+                                 ((tracespec tracespec-p) 'tracespec))
+      :short "Tracing version of @(see eval_subprogram); see @(see
+asl-interpreter-mutual-recursion-*t) for overview."
+      :measure (nats-measure clk 1 0 1)
+      :returns (mv (eval func_eval_result-p) new-orac
+                   (trace asl-tracelist-p))
+      (b* (((mv res orac trace) (eval_subprogram-*t1 env name vparams vargs))
+           (tracespec-entry (cdr (hons-get (identifier-fix name) (tracespec-fix tracespec))))
+           ((unless tracespec-entry)
+            (mv res orac trace))
+           ((tracespec-entry entry) tracespec-entry)
+           (trace (list (make-asl-trace
+                         :fn name
+                         :params (and entry.paramsp vparams)
+                         :args (and entry.argsp vargs)
+                         :globals-in (and entry.globalsp (global-env->storage (env->global env)))
+                         :calls (acl2::rev trace)
+                         :result (if entry.resultp
+                                     res
+                                   (ev_error "Not tracing result" nil nil))))))
+        (mv res orac trace)))))
+
+
+(local
+ (defun add-define-formals (new-formals x)
+   (if (atom x)
+       x
+     (case-match x
+       (('define name formals . rest)
+        `(define ,name ,(append formals new-formals) . ,rest))
+       (& (cons (add-define-formals new-formals (car x))
+                (add-define-formals new-formals (cdr x))))))))
+ 
+
+
+(local (xdoc::set-default-parents asl-interpreter-mutual-recursion-*t))
+
+;; ---------------------------------------------------------------------------
+;; Definition of the Tracing ASL Interpreter (suffixed with *t)
+(make-event
+ (b* ((form *asl-interpreter-mutual-recursion-command*)
+      ;; Strip out the events after the /// (theorem about resolved-p-of-resolve-ty)
+      (form (strip-post-/// form))
+      ;; Strip out xdoc
+      (form (strip-xdoc form))
+      ;; Add xdoc topic for mutual recursion
+      (form (add-mutrec-xdoc *asl-*t-xdoc* form))
+      ;; Add xdoc topic for each function
+      (form (add-define-xdoc
+             "Tracing version of @(see <NAME>); see @(see asl-interpreter-mutual-recursion-*t) for overview."
+             form))
+      ;; Replace '(define eval_subprogram ...' with '(define eval_subprogram-*ft1'
+      ;; since it's going to be wrapped in a call that deals with collecting the trace data.
+      (form (find-eval_subprogram-def-and-rename '*t form))
+      ;; Substitute function names with their -*t suffixed forms.
+      (form (sublis *eval-trace-substitution* form))
+      ;; Wrap each define body in a call of evbody-*ft.
+      (form (wrap-define-bodies 'evbody-*ft form))
+      ;; Add (trace asl-tracelist-p) to all the :returns forms.
+      (form (add-trace-to-returns form))
+      ;; Add the tracespec formal to each define form.
+      (form (add-define-formals '(((tracespec tracespec-p) 'tracespec)) form))
+      ;; Add the definition of eval_subprogram-*t which wraps around eval_subprogram-*t1.
+      (form (add-define-to-defines *eval_subprogram-*t-def* form))
+      ;; Disable the functions, prove the non-trace return values equal to the originals, and verify guards.
+      (form (insert-after-///
+             (list
+              '(make-event
+                `(in-theory (disable . ,(fgetprop 'eval_expr-*t-fn 'acl2::recursivep nil (w state)))))
+              (equals-original-thm '*t (w state))
+              '(verify-guards eval_expr-*t-fn))
+             form)))
+   form))
+;; ---------------------------------------------------------------------------
